clightlight/Clight_Mem0.v
@@ -1,0 +1,292 @@
+Require Import Coqlib.
+Require Import ITreelib.
+Require Import Skeleton.
+Require Import PCM.
+Require Import STS Behavior.
+Require Import Any.
+Require Import ModSem.
+Require Import AList.
+Require Import ConvC2ITree.
+
+From compcert Require Import
+     AST Maps Globalenvs Memory Values Linking Integers.
+From compcert Require Import
+     Ctypes Clight Clightdefs.
+
+Set Implicit Arguments.
+
+Section PROOF.
+
+  Section BODY.
+    Context {Es: Type -> Type}.
+    Context `{has_pE: pE -< Es}.
+    Context `{has_eventE: eventE -< Es}.
+    Context {has_callE: callE -< Es}.
+
+    (* low level allocation of memory *)
+    Definition sallocF: Z * Z -> itree Es val :=
+      fun varg =>
+        mp0 <- trigger (PGet);;
+        m0 <- mp0↓?;;
+        let (lo, hi) := varg in
+        let (m1, blk) := Mem.alloc m0 lo hi in
+        trigger (PPut m1↑);;;
+        Ret (Vptr blk (Ptrofs.repr 0)).
+
+    Definition sfreeF: block * Z * Z -> itree Es unit :=
+      fun varg =>
+        mp0 <- trigger (PGet);;
+        m0 <- mp0↓?;;
+        let '(b, lo, hi) := varg in
+        m1 <- (Mem.free m0 b lo hi)?;;
+        trigger (PPut m1↑);;;
+        Ret tt
+    .
+
+    Definition loadF: memory_chunk * val -> itree Es val :=
+      fun varg =>
+        mp0 <- trigger (PGet);;
+        m0 <- mp0↓?;;
+        let '(chunk, addr) := varg in
+        v <- (Mem.loadv chunk m0 addr)?;;
+        Ret v
+    .
+
+    Definition loadbytesF: val * Z -> itree Es (list memval) :=
+      fun varg =>
+        mp0 <- trigger (PGet);;
+        m0 <- mp0↓?;;
+        let '(addr, n) := varg in
+        match addr with
+        | Vptr b ofs =>
+            v <- (Mem.loadbytes m0 b (Ptrofs.unsigned ofs) n)?;;
+            Ret v
+        | _ => triggerUB
+        end
+    .
+
+    Definition storeF: memory_chunk * val * val -> itree Es unit :=
+      fun varg =>
+        mp0 <- trigger (PGet);;
+        m0 <- mp0↓?;;
+        let '(chunk, addr, v) := varg in
+        m1 <- (Mem.storev chunk m0 addr v)?;;
+        trigger (PPut m1↑);;;
+        Ret tt
+    .
+
+    Definition storebytesF: val * list memval -> itree Es unit :=
+      fun varg =>
+        mp0 <- trigger (PGet);;
+        m0 <- mp0↓?;;
+        let '(addr, bytes) := varg in
+        match addr with
+        | Vptr b ofs =>
+            m1 <- (Mem.storebytes m0 b (Ptrofs.unsigned ofs) bytes)?;;
+            trigger (PPut m1↑);;;
+            Ret tt
+        | _ => triggerUB
+        end
+    .
+
+    Definition valid_pointerF: block * Z -> itree Es bool :=
+      fun varg =>
+        mp0 <- trigger (PGet);;
+        m0 <- mp0↓?;;
+        let '(b, ofs) := varg in
+        Ret (Coqlib.proj_sumbool (Mem.perm_dec m0 b ofs Cur Nonempty))
+    .
+
+    Definition mallocF: list val -> itree Es val :=
+      fun varg =>
+        mp0 <- trigger (PGet);;
+        m0 <- mp0↓?;;
+        '(m1, b) <- (match Archi.ptr64, varg with
+                    | true, [Vlong i] =>
+                        Ret (Mem.alloc m0 (- size_chunk Mptr) (Int64.unsigned i))
+                    | false, [Vint i] =>
+                        Ret (Mem.alloc m0 (- size_chunk Mptr) (Int.unsigned i))
+                    | _, _ => triggerUB
+                    end);;
+        v <- (hd_error varg)?;;
+        m2 <- (Mem.store Mptr m1 b (- size_chunk Mptr) v)?;;
+        trigger (PPut m2↑);;;
+        Ret (Vptr b Ptrofs.zero)
+    .
+
+    Definition freeF: list val -> itree Es val :=
+      fun varg =>
+        mp0 <- trigger (PGet);;
+        m0 <- mp0↓?;;
+        match Archi.ptr64, varg with
+        | _, [Vptr b ofs] =>
+            v_sz <- (Mem.load Mptr m0 b (Ptrofs.unsigned ofs - size_chunk Mptr))?;;
+            let sz := match Archi.ptr64, v_sz with
+                      | true, Vlong i =>
+                          Int64.unsigned i
+                      | false, Vint i =>
+                          Int.unsigned i
+                      | _, _ => (- 1)%Z
+                      end in
+            if (sz >? 0)%Z
+            then m1 <- (Mem.free m0 b (Ptrofs.unsigned ofs - size_chunk Mptr) (Ptrofs.unsigned ofs + sz))?;;
+                 trigger (PPut m1↑);;;
+                 Ret Vundef
+            else triggerUB
+        | true, [Vlong (Int64.mkint 0 _)] => Ret Vundef
+        | false, [Vint (Int.mkint 0 _)] => Ret Vundef
+        | _, _ => triggerUB
+        end
+    .
+    
+    Definition reallocF: list val -> itree Es val :=
+      fun varg =>
+        match varg with
+        | [addr;v_sz'] =>
+            match Archi.ptr64, addr with
+            | true, Vlong (Int64.mkint 0 _)
+            | false, Vint (Int.mkint 0 _) => ccallU "malloc" [v_sz']
+            | _, Vptr b ofs =>
+                (* Read the size of the allocated memory *)
+                mp0 <- trigger (PGet);;
+                m0 <- mp0↓?;;
+                v_sz <- (Mem.load Mptr m0 b (Ptrofs.unsigned ofs - size_chunk Mptr)%Z)?;;
+                let sz := match Archi.ptr64, v_sz with
+                      | true, Vlong i =>
+                          Int64.unsigned i
+                      | false, Vint i =>
+                          Int.unsigned i
+                      | _, _ => (- 1)%Z
+                      end in
+                let sz' := match Archi.ptr64, v_sz' with
+                      | true, Vlong i =>
+                          Int64.unsigned i
+                      | false, Vint i =>
+                          Int.unsigned i
+                      | _, _ => (- 1)%Z
+                      end in
+                if (sz >=? 0)%Z && (sz' >=? 0)%Z
+                then
+                    (* if (sz >=? sz')%Z then (* Reducing the size of the allocated memory *) *)
+                    (*      `_: () <- ccallU "free" (b, sz', sz);; *)
+                    (*          `_: () <- ccallU "store" (Mptr, b, (- size_chunk Mptr)%Z, Vlong (Int64.repr sz'));; *)
+                    (*          Ret (Vptr b (Ptrofs.repr ofs)) *)
+                    (*    else (* Increasing the size of the allocated memory *) *)
+                    `addr': val <- ccallU "malloc" [v_sz'];;
+                    `data: list memval <- ccallU "loadbytes" (addr, sz);;
+                    `_: () <- ccallU "free" [addr];;
+                    `_: () <- ccallU "storebytes" (addr', firstn (Z.to_nat sz') data);;
+                    Ret addr'
+                else triggerUB (* Behaviours vary depending on implementations *)
+            | _, _ => triggerUB
+            end
+        | _ => triggerUB
+        end.
+    
+  End BODY.
+
+  Variable sk: Sk.t.
+  Let skenv: SkEnv.t := Sk.load_skenv sk.
+
+  Definition store_init_data (m : mem) (b : block) (p : Z) (id : init_data) :=
+    match id with
+    | Init_int8 n => Mem.store Mint8unsigned m b p (Vint n)
+    | Init_int16 n => Mem.store Mint16unsigned m b p (Vint n)
+    | Init_int32 n => Mem.store Mint32 m b p (Vint n)
+    | Init_int64 n => Mem.store Mint64 m b p (Vlong n)
+    | Init_float32 n => Mem.store Mfloat32 m b p (Vsingle n)
+    | Init_float64 n => Mem.store Mfloat64 m b p (Vfloat n)
+    | Init_space _ => Some m
+    | Init_addrof symb ofs =>
+        match SkEnv.id2blk skenv (string_of_ident symb) with
+        | Some b' => Mem.store Mptr m b p (Vptr (Pos.of_nat (S b')) ofs)
+        | None => None
+        end
+    end.
+
+
+  Fixpoint store_init_data_list (m : mem) (b : block) (p : Z) (idl : list init_data) {struct idl} : option mem :=
+    match idl with
+    | [] => Some m
+    | id :: idl' =>
+        match store_init_data m b p id with
+        | Some m' => store_init_data_list m' b (p + init_data_size id)%Z idl'
+        | None => None
+        end
+    end.
+  
+  Definition alloc_global (m : mem) (idg : string * C_SkelEntry) :=
+    let (_, g) := idg in
+    match g with
+    | Cgfun _ => let (m1, b) := Mem.alloc m 0 1 in Mem.drop_perm m1 b 0 1 Nonempty
+    | Cgvar v =>
+        let init := gvar_init v in
+        let sz := init_data_list_size init in
+        let (m1, b) := Mem.alloc m 0 sz in
+        match store_zeros m1 b 0 sz with
+        | Some m2 =>
+            match store_init_data_list m2 b 0 init with
+            | Some m3 => Mem.drop_perm m3 b 0 sz (Genv.perm_globvar v)
+            | None => None
+            end
+        | None => None
+        end
+    end.
+      
+
+  Fixpoint alloc_globals (m: mem) (gl: list (string * C_SkelEntry))
+                       {struct gl} : option mem :=
+  match gl with
+  | nil => Some m
+  | g :: gl' =>
+      match alloc_global m g with
+      | None => None
+      | Some m' => alloc_globals m' gl'
+      end
+  end.
+
+  Fixpoint unfold_skel (sk: Sk.t) : option (list (string * C_SkelEntry)) :=
+    match sk with
+    | [] => Some []
+    | (ident, any) :: t =>
+        match Any.downcast any with
+        | Some d => match unfold_skel t with Some t' => Some ((ident, d) :: t') | None => @None (list (string * C_SkelEntry)) end
+        | _ => @None (list (string * C_SkelEntry))
+        end
+    end.
+
+  Definition load_mem :=
+    match unfold_skel sk with
+    | Some gl =>
+        match alloc_globals Mem.empty gl with
+        | Some m => m
+        | None => Mem.empty
+        end
+    | None => Mem.empty
+    end.
+  
+  Definition MemSem : ModSem.t :=
+    {|
+      ModSem.fnsems := [("salloc", cfunU sallocF); ("sfree", cfunU sfreeF);
+                        ("load", cfunU loadF); ("loadbytes", cfunU loadbytesF);
+                        ("store", cfunU storeF); ("storebytes", cfunU storebytesF);
+                        ("malloc", cfunU mallocF); ("free", cfunU freeF); 
+                       (*  ("realloc", cfunU reallocF); *)
+                        ("valid_pointer", cfunU valid_pointerF)];
+      ModSem.mn := "Mem";
+      ModSem.initial_st := (load_mem)↑;
+    |}
+  .
+  
+End PROOF.
+
+Definition size_t := if Archi.ptr64 then tulong else tuint.
+
+Definition Mem: Mod.t :=
+  {|
+    Mod.get_modsem := MemSem;
+    Mod.sk := [("malloc", (Cgfun (Tfunction (Tcons size_t Tnil) (tptr tvoid) cc_default))↑);
+               ("free", (Cgfun (Tfunction (Tcons (tptr tvoid) Tnil) tvoid cc_default))↑)]
+(*                ("realloc", (Cgfun (Tfunction (Tcons (tptr tvoid) (Tcons size_t Tnil)) (tptr tvoid) cc_default))↑)] *)
+  |}
+.
