clightlight/Clightlight2ClightArith.v
@@ -1,0 +1,130 @@
+From compcert Require Import Globalenvs Smallstep AST Integers Events Behaviors Errors Memory.
+Require Import Coqlib.
+Require Import ITreelib.
+Require Import Skeleton.
+Require Import PCM.
+Require Import STS Behavior.
+Require Import Any.
+Require Import ModSem.
+
+Require Import Clightlight2ClightMatch.
+Require Import Clightlight2ClightGenv.
+
+From compcert Require Import Csharpminor.
+
+Set Implicit Arguments.
+
+Ltac unfold_Int64_modulus := unfold Int64.modulus, Int64.wordsize, Wordsize_64.wordsize in *.
+Ltac unfold_Int64_max_signed := unfold Int64.max_signed, Int64.half_modulus in *; unfold_Int64_modulus.
+Ltac unfold_Int64_min_signed := unfold Int64.min_signed, Int64.half_modulus in *; unfold_Int64_modulus.
+Ltac unfold_Ptrofs_modulus := unfold Ptrofs.modulus, Ptrofs.wordsize, Wordsize_Ptrofs.wordsize in *.
+Ltac unfold_Ptrofs_half_modulus := unfold Ptrofs.half_modulus in *; unfold_Ptrofs_modulus.
+Ltac unfold_Int_modulus := unfold Int.modulus, Int.wordsize, Wordsize_32.wordsize in *.
+Ltac unfold_Int_max_signed := unfold Int.max_signed, Int.half_modulus in *; unfold_Int_modulus.
+Ltac unfold_Int_min_signed := unfold Int.min_signed, Int.half_modulus in *; unfold_Int_modulus.
+
+Section ARITH.
+
+  Context `{Σ: GRA.t}.
+  Context `{builtins : builtinsTy}.
+
+  Lemma int64_ptrofs :
+    Ptrofs.modulus = Int64.modulus.
+  Proof. unfold_Int64_modulus. unfold_Ptrofs_modulus. des_ifs. Qed.
+
+  Lemma int64_ext
+        i0 i1
+        (INTVAL: (Int64.intval i0) = (Int64.intval i1))
+    :
+      i0 = i1.
+  Proof.
+    destruct i0, i1. ss. clarify. f_equal. apply proof_irrelevance.
+  Qed.
+
+  Lemma int64_mod_ext
+        i0 i1
+        (INTVAL: ((Int64.intval i0) mod Int64.modulus)%Z = ((Int64.intval i1) mod Int64.modulus)%Z)
+    :
+      i0 = i1.
+  Proof.
+    destruct i0, i1. ss. rewrite Z.mod_small in INTVAL; try lia. rewrite Z.mod_small in INTVAL; try lia.
+    eapply int64_ext; eauto.
+  Qed.
+
+  Lemma ptrofs_ext
+        i0 i1
+        (INTVAL: (Ptrofs.intval i0) = (Ptrofs.intval i1))
+    :
+      i0 = i1.
+  Proof.
+    destruct i0, i1. ss. clarify. f_equal. apply proof_irrelevance.
+  Qed.
+
+  Lemma ptrofs_mod_ext
+        i0 i1
+        (INTVAL: ((Ptrofs.intval i0) mod Ptrofs.modulus)%Z = ((Ptrofs.intval i1) mod Ptrofs.modulus)%Z)
+    :
+      i0 = i1.
+  Proof.
+    destruct i0, i1. ss. rewrite Z.mod_small in INTVAL; try lia. rewrite Z.mod_small in INTVAL; try lia.
+    eapply ptrofs_ext; eauto.
+  Qed.
+
+  Lemma map_val_addl_comm
+        defs a b v
+        (VADD: Values.Val.addl a b = v)
+    :
+      Values.Val.addl (map_val defs a) (map_val defs b) = (map_val defs v).
+  Proof.
+  Admitted.
+
+  Lemma map_val_add_comm
+        defs a b v
+        (VADD: Values.Val.add a b = v)
+    :
+      Values.Val.add (map_val defs a) (map_val defs b) = (map_val defs v).
+  Proof.
+  Admitted.
+
+  Lemma map_val_sub_comm
+        defs a b v
+        (VADD: Values.Val.sub a b = v)
+    :
+      Values.Val.sub (map_val defs a) (map_val defs b) = (map_val defs v).
+  Proof.
+  Admitted.
+
+  Lemma map_val_subl_comm
+        defs a b v
+        (VADD: Values.Val.subl a b = v)
+    :
+      Values.Val.subl (map_val defs a) (map_val defs b) = (map_val defs v).
+  Proof.
+  Admitted.
+
+  Lemma map_val_mul_comm
+        defs a b v
+        (VADD: Values.Val.mul a b = v)
+    :
+      Values.Val.mul (map_val defs a) (map_val defs b) = (map_val defs v).
+  Proof.
+  Admitted.
+
+  Lemma map_val_mull_comm
+        defs a b v
+        (VADD: Values.Val.mull a b = v)
+    :
+      Values.Val.mull (map_val defs a) (map_val defs b) = (map_val defs v).
+  Proof.
+  Admitted.
+
+(*   Lemma map_val_div_comm
+        defs a b v
+        (VADD: Values.Val.div a b = v)
+    :
+      Values.Val.div (map_val defs a) (map_val defs b) = (map_val defs v).
+  Proof.
+  Admitted. *)
+
+End ARITH.
+
