clightlight/Clightlight2ClightGenv.v
@@ -1,0 +1,111 @@
+From compcert Require Import Maps Globalenvs Smallstep AST Integers Events Behaviors Errors Memory.
+From ExtLib Require Import Data.List.
+Require Import Coqlib.
+Require Import ITreelib.
+Require Import Skeleton.
+Require Import PCM.
+Require Import STS Behavior.
+Require Import Any.
+Require Import ModSem.
+Require Import AList.
+
+Require Import ConvC2ITree.
+Require Import Clightlight2ClightMatch.
+
+From compcert Require Import Ctypes Clight Clightdefs.
+
+Import Permutation.
+
+Set Implicit Arguments.
+
+Section GENV.
+
+  Context `{Σ: GRA.t}.
+
+  Variable types : list composite_definition.
+  Variable defs : list (ident * globdef fundef type).
+  Variable WF_TYPES : wf_composites types.
+  Variable sge : alist string Any.t.
+  Let ce := let (ce, _) := build_composite_env' types WF_TYPES in ce.
+
+  Lemma found_itree_clight_function
+        (fn: string) 
+        (i: list Values.val -> itree Es Values.val) 
+        (mn: string) (p: ident)
+        (FOUND : find
+                    ((fun '(k2, _) => fn ?[ eq ] k2) <*>
+                     map_snd
+                      (fun sem => transl_all mn (T:=Any.t) ∘ sem) <*>
+                     (fun '(fn, f) => (string_of_ident fn, cfunU f)))
+                    (decomp_fundefs types WF_TYPES sge defs) = 
+                 Some (p, i))
+    :
+      (ident_of_string fn = p) /\ (In (p, i) (decomp_fundefs types WF_TYPES sge defs)).
+  Proof.
+    apply find_some in FOUND. des. split; auto.
+    unfold compose in FOUND0. simpl in FOUND0. rewrite eq_rel_dec_correct in FOUND0. des_ifs.
+  Admitted.
+
+  Lemma decomp_fundefs_decomp_func i p
+        (INLEFT: In (p, i) (decomp_fundefs types WF_TYPES sge defs)) 
+    :
+        exists f, i = decomp_func sge ce f /\ In (p, Gfun (Internal f)) defs.
+  Proof.
+    induction defs.
+    { inv INLEFT. }
+    destruct a as [? [[|]|]].
+    2, 3: apply IHl in INLEFT; des; simpl; eauto.
+    simpl in INLEFT. des.
+    2: apply IHl in INLEFT; des; simpl; eauto.
+    inv INLEFT. simpl. eexists; split; eauto.
+  Qed.  
+  
+  Lemma in_def_gdefs a clight_prog
+        (INDEFS_FUN: In a defs)
+        (RIGHT_COMP: clight_prog = mkprogram types defs (List.map (fun '(gn, _) => gn) defs) (ident_of_string "main") WF_TYPES)
+    :
+        In a clight_prog.(prog_defs).
+  Proof.
+    unfold mkprogram, build_composite_env' in *. des_ifs.
+  Qed.
+
+  Lemma tgt_genv_match_symb_def
+        clight_prog name b gd1 gd2
+        (NO_REP: Coqlib.list_norepet (List.map fst defs))
+        (RIGHT_COMP: clight_prog = mkprogram types defs (List.map (fun '(gn, _) => gn) defs) (ident_of_string "main") WF_TYPES)
+        (GFSYM: Genv.find_symbol (Genv.globalenv clight_prog) (ident_of_string name) = Some b)
+        (GFDEF: Genv.find_def (Genv.globalenv clight_prog) b = Some gd1)
+        (INTGT: In (ident_of_string name, gd2) (prog_defs clight_prog))
+    :
+      gd1 = gd2.
+  Proof.
+    assert (AST.prog_defs clight_prog = defs) by now
+      unfold mkprogram, build_composite_env' in *; des_ifs.
+    assert (prog_defs clight_prog = defs) by now
+      unfold mkprogram, build_composite_env' in *; des_ifs.
+    hexploit prog_defmap_norepet.
+    { unfold prog_defs_names. rewrite H. auto. }
+    { eauto. }
+    i. apply Genv.find_def_symbol in H1. des. clarify.
+  Qed.
+
+  Lemma tgt_genv_find_def_by_blk
+        clight_prog name b gd 
+        (NO_REP: Coqlib.list_norepet (List.map fst defs))
+        (RIGHT_COMP: clight_prog = mkprogram types defs (List.map (fun '(gn, _) => gn) defs) (ident_of_string "main") WF_TYPES)
+        (GFSYM: Genv.find_symbol (Genv.globalenv clight_prog) (ident_of_string name) = Some b)
+        (INTGT: In (ident_of_string name, gd) (prog_defs clight_prog))
+    :
+      Genv.find_def (Genv.globalenv clight_prog) b = Some gd.
+  Proof.
+    assert (AST.prog_defs clight_prog = defs) by now
+      unfold mkprogram, build_composite_env' in *; des_ifs.
+    assert (prog_defs clight_prog = defs) by now
+      unfold mkprogram, build_composite_env' in *; des_ifs.
+    hexploit prog_defmap_norepet.
+    { unfold prog_defs_names. rewrite H. auto. }
+    { eauto. }
+    i. apply Genv.find_def_symbol in H1. des. clarify.
+  Qed.
+
+End GENV.
