clightlight/Clightlight2ClightLenv.v
@@ -1,0 +1,104 @@
+From compcert Require Import Maps Clight Clightdefs.
+From ExtLib Require Import Data.List.
+Require Import Coqlib.
+Require Import PCM.
+Require Import AList.
+
+Require Import Clightlight2ClightMatch.
+
+Set Implicit Arguments.
+
+Section LENV.
+
+  Context `{Σ: GRA.t}.
+  Context `{builtins : builtinsTy}.
+
+  Lemma update_le
+        defs x id v sv le tle
+        (SRC_UPDATE: Maps.PTree.get x (Maps.PTree.set id v tle) = Some sv)
+        (MLE: match_le defs le tle)
+    :
+      Maps.PTree.get x (Maps.PTree.set id (map_val defs v) tle) = Some (map_val defs sv).
+  Proof.
+  Admitted.
+
+  Lemma bind_parameter_temps_exists_if_same_length
+        params args tle0
+        (LEN: List.length params = List.length args)
+    :
+      exists tle, (<<BIND: bind_parameter_temps params args tle0 = Some tle>>).
+  Proof.
+    depgen args. depgen tle0. clear. induction params; i; ss; clarify.
+    { exists tle0. des_ifs. }
+    destruct args; ss; clarify. destruct a. eauto.
+  Qed.
+
+  Lemma bind_parameter_temps_exists
+        defs base params sle rvs (tle0: temp_env)
+        (BIND_SRC: bind_parameter_temps params rvs base = Some sle)
+    :
+      exists tle, (<<BIND_TGT: bind_parameter_temps params (List.map (map_val defs) rvs) tle0
+                      = Some tle>>).
+  Proof.
+    eapply bind_parameter_temps_exists_if_same_length; eauto.
+    rewrite ! map_length. clear -BIND_SRC. depgen base. revert sle.  depgen rvs. depgen params.
+    induction params; i; ss; des_ifs.
+    ss. f_equal. eapply IHparams; eauto.
+  Qed.
+
+(*   Lemma init_lenv_match
+        src le tle l
+        (SINIT: le = init_lenv l)
+        (TINIT: tle = create_undef_temps (List.map s2p l))
+    :
+      <<MLINIT: match_le src le tle >>.
+  Proof.
+    red. depgen src. depgen le. depgen tle. clear. induction l; ii; ss; clarify.
+    match goal with
+    | [ |- match_le _ (_ :: ?_le0) (PTree.set _ _ ?_tle0)] => specialize IHl with (tle:=_tle0) (le:=_le0) (src:=src) end.
+    hexploit IHl; eauto. clear IHl. i. inv H.
+    econs. i. ss. des_ifs.
+    { rewrite eq_rel_dec_correct in Heq. des_ifs. rewrite PTree.gss. ss. }
+    apply neg_rel_dec_correct in Heq.
+    rewrite PTree.gso; eauto. ii. apply Heq. apply s2p_inj in H0. ss.
+  Qed. *)
+
+  (*** TODO: lenv initialization has match ***)
+(*   Lemma _initial_lenv_match
+        src params rvs le0 le (tle0: temp_env) tle
+        (ML0: match_le src le0 tle0)
+        (ARGS: init_args params rvs le0 = Some le)
+        (BIND: bind_parameters (List.map s2p params)
+                               (List.map (map_val src) rvs) tle0
+               = Some tle)
+    :
+      (<<MLINIT: match_le src le tle>>).
+  Proof.
+    red. move params before builtins. revert_until params. clear. induction params; i; ss; clarify.
+    { destruct rvs; ss; clarify. }
+    destruct rvs eqn:RVS; ss; clarify.
+    eapply IHparams.
+    2: eapply ARGS.
+    2: eapply BIND.
+    depgen ML0. clear; i. econs; i. eapply alist_update_le; eauto.
+  Qed.
+
+  Lemma initial_lenv_match
+        src impf rvs le0 le (tle0: temp_env)
+        (SINIT: le0 = init_lenv (impf.(Imp.fn_vars) ++ ["return"; "_"]))
+        (ARGS: init_args impf.(Imp.fn_params) rvs le0 = Some le)
+        (TINIT: tle0 = create_undef_temps
+                         (List.map (fun vn : string => s2p vn) (impf.(Imp.fn_vars) ++ ["return"; "_"])))
+    :
+      exists tle, (<<BIND: bind_parameters
+                        (List.map (fun vn : string => s2p vn) impf.(Imp.fn_params))
+                        (List.map (map_val src) rvs) tle0 = Some tle>>) /\
+             (<<MLINIT: match_le src le tle>>).
+  Proof.
+    hexploit bind_parameters_exists; eauto. i. des.
+    exists tle. split; eauto.
+    eapply _initial_lenv_match; eauto.
+    eapply init_lenv_match; eauto.
+  Qed. *)
+
+End LENV.
