clightlight/Clightlight2ClightMatch.v
@@ -1,0 +1,266 @@
+From compcert Require Import Globalenvs Smallstep AST Integers Events Behaviors Errors Memory Values Maps.
+Require Import Coqlib.
+Require Import ITreelib.
+Require Import Skeleton.
+Require Import PCM.
+Require Import STS Behavior.
+Require Import Any.
+Require Import ModSem.
+Require Import ConvC2ITree.
+Require Import Clight_Mem0.
+
+Set Implicit Arguments.
+
+From compcert Require Import Ctypes Clight Clightdefs.
+
+Section MATCH.
+
+  Fixpoint get_cont_stmts (cc: cont) : list statement :=
+    match cc with
+    | Kseq s k => s :: (get_cont_stmts k)
+    | _ => []
+    end
+  .
+
+(*   Fixpoint wf_ccont (k: cont) : Prop :=
+    match k with
+    | Kseq s k2 =>
+      match s with
+      | Sreturn _ =>
+        match k2 with
+        | Kstop => True
+        | Kcall _ _ env _ k3 => (env = empty_env /\ wf_ccont k3)
+        | _ => False
+        end
+      | _ => wf_ccont k2
+      end
+    | _ => False
+    end
+  . *)
+
+  Fixpoint get_cont_stack k : option cont :=
+    match k with
+    | Kseq s k2 => get_cont_stack k2
+    | Kcall _ _ _ _ _ => Some k
+    | _ => None 
+    end
+  .
+(*
+  Lemma wf_cont_has_stack
+        k
+        (WFCCONT: wf_ccont k)
+    :
+      exists ks, get_cont_stack k = Some ks.
+  Proof.
+    revert_until k.
+    induction k; i; ss; clarify.
+    destruct s; ss; clarify; eauto.
+    destruct k; ss; clarify; eauto.
+  Qed. *)
+
+  Context `{Σ: GRA.t}.
+  
+  Definition itree_of_Es_format {A} (es_itree: itree Es A) (ms: ModSemL.t) (mn: string) (rp: p_state) :=
+     EventsL.interp_Es (ModSemL.prog ms) (transl_all mn es_itree) rp.
+
+  (* Definition itree_of_stmt (sk: Sk.t) (ce: composite_env) (ms: ModSem.t) (mn: string) (retty: type) :=
+    fun code e le rp =>
+     itree_of_Es_format (decomp_stmt sk ce retty code e le) ms mn rp.
+
+  Fixpoint itree_of_stmts (sk: Sk.t) (ce: composite_env) (ms: ModSem.t) (mn: string) (retty: type) (stmts: list statement) :=
+    match stmts with
+    | [] => (fun e le p => Ret (p, (e, le, None, ))
+    | a :: l =>
+          fun e le p =>
+            ((p', (e', le', bc, v)) <- (itree_of_stmt sk ce ms mn retty a e le p);;
+            match v with
+            | Some retval =>
+              Ret (e', le', None, v)
+            | None =>
+              match bc with
+              | None =>
+                (itree_of_stmts sk ce ms mn l retty e' le' p')
+              | Some _ => Ret (e', le', bc, None)
+              end
+            end)
+    end.
+    itree_of_stmt
+    fun sk ce rettype code e le ms mn rp =>
+      EventsL.interp_Es (ModSemL.prog ms) (transl_all mn (decomp_stmt sk ce rettype code e le)) rp. *)
+(*
+  Definition itree_of_imp_ret :=
+    fun ge le ms mn rp =>
+      itree_of_imp_cont (denote_expr (Var "return"%string)) ge le ms mn rp.
+
+  Lemma itree_of_imp_cont_bind
+        T R ge le ms mn rp (itr: itree _ T) (ktr: T -> itree _ R)
+    :
+      itree_of_imp_cont (x <- itr;; ktr x) ge le ms mn rp
+      =
+      '(p, (le2, v)) <- (itree_of_imp_cont itr ge le ms mn rp);; (itree_of_imp_cont (ktr v) ge le2 ms mn (p)).
+  Proof.
+    unfold itree_of_imp_cont. rewrite interp_imp_bind. grind.
+    rewrite! transl_all_bind; rewrite! EventsL.interp_Es_bind.
+    grind. destruct p0. grind.
+  Qed.
+
+  Definition itree_of_imp_pop :=
+    fun ge ms mn retmn (retx: var) (retle: lenv) (x: _ * (lenv * val)) =>
+      let '(p, (le0, _)) := x in
+      '(p2, rv) <- EventsL.interp_Es (ModSemL.prog ms) (transl_all mn ('(_, v) <- interp_imp ge (denote_expr (Var "return"%string)) le0;; Ret (v↑))) (p);;
+      '(p3, rv) <- EventsL.interp_Es (ModSemL.prog ms) ((tau;; Ret rv)) (p2);;
+      pop <- EventsL.interp_Es (ModSemL.prog ms) (transl_all retmn (tau;; tau;; v0 <- unwrapU (rv↓);; (tau;; tau;; tau;; Ret (alist_add retx v0  retle, Vundef)))) (p3);;
+      Ret pop.
+
+  Definition itree_of_imp_pop_bottom :=
+    fun ms mn (x : p_state * (lenv * val)) =>
+      ` x0 : p_state * Any.t <-
+      (let (st1, v) := x in
+      EventsL.interp_Es (ModSemL.prog ms)
+                        (transl_all mn (` x0 : val <- (let (_, retv) := v in Ret retv);; Ret (Any.upcast x0))) st1);; Ret (snd x0).
+
+  Definition itree_of_cont_stmt (s : Imp.stmt) :=
+    fun ge le ms mn rp => itree_of_imp_cont (denote_stmt s) ge le ms mn rp.
+
+  Definition imp_state := itree eventE Any.t.
+  Definition imp_cont {T} {R} := (p_state * (lenv * T)) -> itree eventE (p_state * (lenv * R)).
+  Definition imp_stack := (p_state * (lenv * val)) -> imp_state.
+
+  (* Hypothesis archi_ptr64 : Archi.ptr64 = true. *)
+  Context `{builtins : builtinsTy}.
+
+  Definition ext_len : Imp.programL -> nat := fun src => List.length (src.(ext_varsL)) + List.length (src.(ext_funsL)).
+  Definition int_len : Imp.programL -> nat := fun src => List.length (src.(prog_varsL)) + List.length (src.(prog_funsL)).
+  Definition sk_len : Imp.programL -> nat := fun src => List.length src.(defsL).
+  (* next block of src's initialized genv *)
+  Definition src_init_nb : Imp.programL -> nat := fun src => sk_len src.
+  (* next block of tgt's initialized genv *)
+  Definition tgt_init_len := List.length ((@init_g builtins) ++ c_sys).
+  Definition tgt_init_nb : Imp.programL -> Values.block := fun src => Pos.of_succ_nat (tgt_init_len + (ext_len src) + (int_len src)).
+
+  Definition get_sge (src : Imp.programL) := Sk.load_skenv (Sk.sort (ImpMod.get_modL src).(ModL.sk)).
+  Definition get_tge (tgt : Csharpminor.program) := Genv.globalenv tgt.
+
+ *)
+  (* should never appear *)
+  Definition dummy_blk : positive := 1%positive.
+
+  Definition map_blk (defs: list (AST.ident * AST.globdef Clight.fundef Ctypes.type)) : positive -> Values.block :=
+    fun blk =>
+      if (ge_dec (Pos.to_nat blk) (S (List.length (get_sk defs))))
+      then Pos.of_nat ((List.length defs - List.length (get_sk defs)) + (Pos.to_nat blk))
+      else
+        let sg := Sk.load_skenv (get_sk defs) in
+        let tg := Genv.add_globals (Genv.empty_genv _ _ (List.map fst defs)) defs  in
+        match sg.(SkEnv.blk2id) (pred (Pos.to_nat blk)) with
+        | Some name =>
+          match Genv.find_symbol tg (ident_of_string name) with
+          | Some tblk => tblk
+          | None => dummy_blk
+          end
+        | None => dummy_blk
+        end
+  .
+
+  Definition map_val defs (v : val) : val :=
+    match v with
+    | Vptr blk ofs => Vptr (map_blk defs blk) ofs
+    | _ => v
+    end.
+
+  Definition map_memval defs (mv : memval) : memval :=
+    match mv with
+    | Fragment v q n => Fragment (map_val defs v) q n
+    | _ => mv
+    end.
+
+  Variant match_le defs : temp_env -> temp_env -> Prop :=
+  | match_le_intro
+      sle tle 
+      (ML: forall id sv, Maps.PTree.get id sle = Some sv -> Maps.PTree.get id tle = Some (map_val defs sv))
+    :
+      match_le defs sle tle.
+
+  Variant match_ge defs : SkEnv.t -> (Genv.t fundef ()) -> Prop :=
+  | match_ge_intro
+      sge tge
+      (MG: forall gn idx,
+          (sge.(SkEnv.id2blk) gn = Some idx) ->
+          (Genv.find_symbol tge (ident_of_string gn) = Some (map_blk defs (Pos.of_succ_nat idx))))
+    :
+      match_ge defs sge tge.
+(*
+  Definition return_stmt := Sreturn (Some (Evar (s2p "return"))).
+  Definition ret_call_cont k := Kseq return_stmt (call_cont k).
+
+  Definition exit_stmt := Sreturn (Some (Eunop Cminor.Ointoflong (Evar (s2p "return")))).
+  Definition ret_call_main := Kseq exit_stmt Kstop.
+
+  (* global env is fixed when src program is fixed *)
+  Variable ge : SkEnv.t.
+  (* ModSem should be fixed with src too *)
+  Variable ms : ModSemL.t.
+
+  Inductive match_code (mn: mname) : imp_cont -> (list Csharpminor.stmt) -> Prop :=
+  | match_code_exit
+    :
+      match_code mn (fun '(p, (le, _)) => itree_of_imp_ret ge le ms mn (p)) [exit_stmt]
+  | match_code_return
+    :
+      match_code mn idK [return_stmt]
+  | match_code_cont
+      code itr ktr chead ctail
+      (CST: compile_stmt code = chead)
+      (ITR: itr = fun '(p, (le, _)) => itree_of_cont_stmt code ge le ms mn (p))
+      (MCONT: match_code mn ktr ctail)
+    :
+      match_code mn (fun x => (itr x >>= ktr)) (chead :: ctail)
+  .
+
+  Inductive match_stack (src: Imp.programL) (mn: mname) : imp_stack -> option Csharpminor.cont -> Prop :=
+  | match_stack_bottom
+    :
+      match_stack src mn (itree_of_imp_pop_bottom ms mn) (Some ret_call_main)
+
+  | match_stack_cret
+      tf le tle next stack tcont id tid tpop retmn
+      (MLE: @match_le src le tle)
+      (MID: s2p id = tid)
+
+      (WFCONT: wf_ccont tcont)
+      (MCONT: match_code retmn next (get_cont_stmts tcont))
+      (MSTACK: match_stack src retmn stack (get_cont_stack tcont))
+
+      (TPOP: tpop = ret_call_cont (Kcall (Some tid) tf empty_env tle tcont))
+    :
+      match_stack src mn (fun x => (y <- (itree_of_imp_pop ge ms mn retmn id le x);; next y >>= stack)) (Some tpop)
+  .
+ *)
+
+  Variant match_mem defs : Memory.Mem.mem -> Memory.Mem.mem -> Prop :=
+  | match_mem_intro
+      m tm
+      (INITIALIZED: Pos.to_nat m.(Mem.nextblock) >= (List.length (get_sk defs)))
+      (NBLK: tm.(Mem.nextblock) = map_blk defs (m.(Mem.nextblock)))
+      (MEM_CNT: forall b ofs mv, PMap.get ofs (PMap.get b m.(Mem.mem_contents)) = mv -> PMap.get ofs (PMap.get (map_blk defs b) tm.(Mem.mem_contents)) = map_memval defs mv )
+      (MEM_PERM: forall b, PMap.get b m.(Mem.mem_access) = Maps.PMap.get (map_blk defs b) tm.(Mem.mem_access) )
+    :
+      match_mem defs m tm
+  .
+
+(*   Variant match_states src : imp_state -> Csharpminor.state -> Prop :=
+  | match_states_intro
+      tf pstate le tle code itr tcode m tm next stack tcont mn
+      (CST: compile_stmt code = tcode)
+      (ML: @match_le src le tle)
+      (PSTATE: pstate "Mem"%string = m↑)
+      (MM: @match_mem src m tm)
+      (WFCONT: wf_ccont tcont)
+      (MCONT: next = itree_of_stmts (get_cont_stmts tcont))
+      (MSTACK: @match_stack src mn stack (get_cont_stack tcont))
+      (ITR: body = itree_of_stmt sk ce rettype tcode e le ms mn pstate)
+    :
+      match_states src (x <- body;; next x >>= stack) (State tf tcode tcont te tle tm)
+  . *)
+
+End MATCH.
