clightlight/Clightlight2ClightSepComp.v
@@ -1,0 +1,307 @@
+From compcert Require Import Coqlib Integers Floats AST Ctypes Cop Clight Clightdefs.
+Require Import Coqlib.
+Require Import ITreelib.
+Require Import Skeleton.
+Require Import PCM.
+Require Import STS Behavior.
+Require Import Any.
+Require Import ModSem.
+Require Import SimSTS3.
+Require Import Clight_Mem0.
+Require Import IRed.
+From Ordinal Require Import Ordinal Arithmetic.
+Require Import ConvC2ITree.
+
+Require Import Clightlight2ClightMatch.
+Require Import Clightlight2ClightArith.
+Require Import Clightlight2ClightGenv.
+(* Require Import Clightlight2ClightLenv. *)
+Require Import Clightlight2ClightMem.
+Require Import Clightlight2ClightLink.
+(* Require Import Clightlight2ClightSim.  *)
+
+Section PROOFSINGLE.
+
+  Context `{Σ: GRA.t}.
+  Context `{builtins : builtinsTy}.
+
+  Create HintDb ord_step2.
+  Hint Resolve Nat.lt_succ_diag_r OrdArith.lt_from_nat OrdArith.lt_add_r: ord_step2.
+  Hint Extern 1000 => lia: ord_step2.
+  Ltac ord_step2 := eauto with ord_step2.
+
+  Ltac solve_mkprogram := unfold mkprogram, build_composite_env' in *; des_ifs; eauto.
+
+  Ltac sim_red := try red; Red.prw ltac:(_red_gen) 2 0. (* these are itree normalization tactic *)
+  Ltac sim_tau := (try sim_red); econs 3; ss; clarify; eexists; exists (ModSemL.step_tau _); eexists; split; [ord_step2|auto].
+  (* Ltac sim_triggerUB := unfold triggerUB; (try sim_red); econs 5; i; ss; auto; *)
+  (*                       dependent destruction STEP; try (irw in x; clarify; fail). *)
+  Ltac solve_ub := des; irw in H; dependent destruction H; clarify. (* how to end with ub *)
+  Ltac sim_triggerUB := (try rename H into HH); pfold; ss; unfold triggerUB; try sim_red; econs 5; i; ss; auto;
+                        [solve_ub | dependent destruction STEP; try (irw in x; clarify; fail)].
+
+  Ltac dtm H H0 := eapply angelic_step in H; eapply angelic_step in H0; des; rewrite H; rewrite H0; ss.
+
+(*
+  Definition imp_sem (src : Imp.programL) := compile_val (ModL.add (Mod.lift (Mem (fun _ => false))) (ImpMod.get_modL src)).
+
+  Definition imp_initial_state (src : Imp.programL) := (imp_sem src).(initial_state).
+ *)
+
+(** Why does final value determines sort of state? *)
+(** The reason why Vint is special is just "int main(void)"? *)
+
+  Definition compile_val md := @ModL.compile _ EMSConfigC md. 
+
+  Definition clightligt_sem types defs WF_COMP mn := compile_val (ModL.add (Mod.lift Mem) (Mod.lift (get_mod types defs WF_COMP mn))).
+
+  Definition clightlight_initial_state types defs WF_COMP mn := (clightligt_sem types defs WF_COMP mn).(initial_state).
+  Opaque ident_of_string.
+
+  Definition has_malloc (defs: list (_ * AST.globdef Clight.fundef Ctypes.type)) :=
+     In (ident_of_string "malloc", Gfun (External EF_malloc (Ctypes.Tcons tulong Ctypes.Tnil) (tptr tvoid) cc_default)) defs.
+
+  Definition has_free (defs: list (_ * AST.globdef Clight.fundef Ctypes.type)) :=
+     In (ident_of_string "free", Gfun (External EF_free (Ctypes.Tcons (tptr tvoid) Ctypes.Tnil) tvoid cc_default)) defs.
+
+  
+  Theorem single_compile_behavior_improves
+          (types: list Ctypes.composite_definition)
+          (defs: list (AST.ident * AST.globdef Clight.fundef Ctypes.type))
+          (WF_TYPES: Clightdefs.wf_composites types) mn modl clight_prog
+          (NO_REP: Coqlib.list_norepet (List.map fst defs))
+          (HAS_MALLOC: has_malloc defs)
+          (HAS_FREE: has_free defs)
+          (LEFT_COMP: modl = ModL.add (Mod.lift Mem) (Mod.lift (get_mod types defs WF_TYPES mn)))
+          (RIGHT_COMP: clight_prog = mkprogram types defs (List.map (fun '(gn, _) => gn) defs) (ident_of_string "main") WF_TYPES)
+          left_st right_st
+          (LEFT_INIT: left_st = clightlight_initial_state types defs WF_TYPES mn)
+          (RIGHT_INIT: Clight.initial_state clight_prog right_st)
+        :
+          <<IMPROVES: @improves2 _ (Clight.semantics2 clight_prog) left_st right_st>>.
+  Proof.
+    eapply adequacy; eauto.
+    { apply Ordinal.Ord.lt_well_founded. }
+    { admit "I have to prove well formedness of Clight compile result". }
+    instantiate (1:= (Ord.omega * Ord.omega + Ord.omega + 1)%ord).
+    red. ginit.
+    { instantiate (1:= (cpn3 (_sim (clightligt_sem types defs WF_TYPES mn) (semantics2 clight_prog)))).
+      econs. { red. i. econs.    }  }
+     rewrite LEFT_INIT. unfold clightlight_initial_state in *. ss; clarify. inv RIGHT_INIT.
+    unfold ModSemL.initial_itr.
+    rename ge into tge, H into INIT_MEM, H0 into MAIN_BLOCK, H1 into FIND_MAINF, H2 into MAIN_TYPE, f into tmaindef.
+    gstep. econs 5; eauto; unfold assume. 
+    { ss. grind. dtm H H0. }
+    grind. eapply angelic_step in STEP. des; clarify.
+    eexists; split; [ord_step2|].
+
+    left. unfold ITree.map. sim_red. 
+    set (sge_init:= Sk.sort _) in *.
+    destruct (alist_find "main" _) eqn:FOUNDMAIN; ss; grind; [|sim_triggerUB].
+    repeat match goal with | [ H : false = false |- _ ] => clear H end.
+    
+    rewrite alist_find_find_some in FOUNDMAIN. rewrite find_map in FOUNDMAIN.
+    rewrite find_map in FOUNDMAIN. uo; des_ifs; ss. inv H0. clear H1. 
+    hexploit found_itree_clight_function; eauto. i. des. subst. rewrite string_of_ident_of_string.
+    clear Heq0. rename H0 into FIND_ITREE.
+    hexploit decomp_fundefs_decomp_func; eauto. i. des. rename H0 into FIND_TFUNC.
+    set (_main := prog_main _) in *.
+    assert (_main = ident_of_string "main") by now solve_mkprogram. clearbody _main. subst.
+    hexploit tgt_genv_match_symb_def; [> try (unfold tge in *; solve_mkprogram; fail) ..|]; eauto.
+    { des_ifs. clear Heq. unfold Globalenvs.Genv.find_funct_ptr in *. des_ifs. 
+      unfold tge, mkprogram, build_composite_env' in Heq. des_ifs. clear Heq0.
+      rewrite e in e0. inv e0. eauto. }
+    i. inv H. rename f into tmain. 
+    unfold cfunU. rewrite Any.upcast_downcast. unfold decomp_func. grind.
+    clear Heq. rename x into ce, e into EQ. sim_red.
+    unfold function_entry_c.
+    destruct (id_list_norepet_c _ && id_list_norepet_c _ && id_list_disjoint_c _ _); [|sim_triggerUB].
+    sim_red.
+    induction (fn_vars tmain); cycle 1.
+    { ss. destruct a. unfold ccallU. sim_red; ss. pfold; econs 3; ss; grind.
+      eexists. exists (ModSemL.step_tau _). eexists. 
+     }
+    - ss. sim_red. unfold triggerUB. ired. pfold; econs 5; ss; grind.
+      { i. solve_ub. } 
+      { i. dependent destruction STEP; irw in x; ss. injection x. i. simpl_depind. ss. }
+    - ss. destruct a. unfold ccallU; sim_red. ss. pfold; econs 3; ss; grind.
+      { eexists. exists (ModSemL.step_tau _). eexists.
+        split; ord_step2. left. rewrite Any.upcast_downcast. sim_red.
+        unfold sallocF. sim_red.
+      left. 
+
+(*     assert (MAINPARAM: fn_params smain = []).
+    { depgen Heq. clear. i. remember (fn_params smain) as m. clear Heqm. depgen l. induction m; i; ss; clarify. }
+    rename l into sle, Heq into INITARGS. rewrite MAINPARAM in INITARGS. ss. clarify.
+    rewrite interp_imp_tau. sim_red.
+
+    unfold Genv.find_funct_ptr in TMAIN2. subst tge. rewrite TGTMAIN in TMAIN2. clarify.
+    set (tge:=Genv.globalenv tgt) in *. *)
+    pfold. econs 4; ss. eexists. eexists.
+    { rewrite <- NoDup_norepeat in WF_MAIN. apply Coqlib.list_norepet_app in WF_MAIN; des. subst tmainf.
+      rewrite MAINPARAM in *. eapply step_internal_function; ss; eauto; try econs. }
+    eexists; split; [ord_step2|auto]. left. ss.
+
+    unfold ModL.wf in WF. des.
+
+    pfold. econs 6; ss; eauto. eexists. eexists.
+    { eapply step_seq. }
+    eexists. exists (ModSemL.step_tau _). exists ((100 + max_fuel) + 100 + Ord.omega + 100)%ord. left.
+    rewrite interp_imp_bind. grind. sim_red.
+    assert (MATCHGE: match_ge src (Sk.load_skenv (Sk.sort (ModL.sk (ModL.add (Mem (fun _ => false)) (ImpMod.get_modL src))))) (Genv.globalenv tgt)).
+    { econs. i. simpl in H. rewrite Sk.add_unit_l in H.
+      unfold map_blk. rewrite COMP0. hexploit Sk.env_found_range; eauto. i. unfold src_init_nb, int_len.
+      rewrite <- sksort_same_len in H0. ss. unfold sk_len. des.
+      hexploit (Sk.sort_wf SK). i. rewrite Sk.add_unit_l in H1.
+      apply Sk.load_skenv_wf in H1.
+      apply H1 in H. unfold get_sge. ss. rewrite H. unfold get_tge. des_ifs; try lia.
+      hexploit found_in_src_in_tgt; eauto. i. des. unfold get_tge in H2. clarify.
+    }
+    ss. rewrite Sk.add_unit_l in MATCHGE. rewrite Sk.add_unit_l in WF0.
+
+    unfold imp_sem in *. 
+    eapply match_states_sim; eauto.
+    { apply map_blk_after_init. }
+    { apply map_blk_inj. }
+    ss. rewrite Sk.add_unit_l.
+    match goal with
+    | [ |- match_states ?_ge ?_ms _ _ _ ] => replace _ge with sge; auto
+    end.
+    match goal with
+    | [ |- match_states ?_ge ?_ms _ _ _ ] => set (ms:=_ms) in *
+    end.
+    ss.
+    econs; eauto.
+    { eapply init_lenv_match; eauto. rewrite map_app. ss. }
+    { clarify. }
+    { econs; ss.
+      { unfold src_init_nb, sk_len. rewrite <- sksort_same_len. lia. }
+      { apply Genv.init_mem_genv_next in TMINIT. rewrite <- TMINIT. unfold Genv.globalenv. ss.
+        rewrite Genv.genv_next_add_globals. ss. rewrite Genv_advance_next_length. ss.
+        rewrite length_elements_PTree_norepet; eauto. rewrite map_blk_after_init; eauto.
+        2:{ unfold src_init_nb, sk_len. rewrite <- sksort_same_len. lia. }
+        unfold ext_len. subst tgds.
+        rewrite Pos2Nat.inj_1. rewrite Nat.add_1_r. rewrite <- Pos.of_nat_succ. f_equal.
+        rewrite gdefs_preserves_length. repeat rewrite <- Nat.add_assoc. do 3 f_equal.
+        unfold Sk.wf in SK. ss.
+        rewrite Sk.add_unit_l in SK.
+        hexploit wfprog_defsL_length; eauto. i. des.
+        unfold sk_len in *.
+        match goal with | [ |- _ = ?x ] => replace x with (int_len src) end.
+        { unfold int_len. ss. }
+        rewrite <- sksort_same_len. sym. apply Nat.sub_add. auto.
+      }
+      i. uo; des_ifs. unfold NW in H. clarify. rename s into gn, Heq0 into SGENV.
+      set (tblk:=map_blk src blk) in *. unfold map_ofs in *. rewrite! Z.mul_0_r.
+      hexploit found_gvar_in_src_then_tgt; eauto. i. des. rename H into FOUNDTGV.
+      hexploit Genv.init_mem_characterization; eauto.
+      { unfold Genv.find_var_info. rewrite FOUNDTGV. clarify. }
+      i. des. rename H into TMPERM, H0 into TMPERM0, H1 into TMLSID, H2 into TMLB.
+      subst tblk. inv MATCHGE.
+      assert (SKFOUND: SkEnv.blk2id sge blk = Some gn).
+      { subst sge. Local Transparent Sk.load_skenv. unfold Sk.load_skenv. ss. rewrite SGENV. uo; ss. Local Opaque Sk.load_skenv. }
+      assert (WFSKENV: Sk.wf (defsL src)); auto.
+      apply Sk.sort_wf in WFSKENV. apply Sk.load_skenv_wf in WFSKENV. apply WFSKENV in SKFOUND. clear WFSKENV.
+      apply MG in SKFOUND. apply nth_error_In in SGENV. apply WFPROG2 in SGENV.
+      hexploit compiled_gvar_props; eauto. i. des. clarify.
+      assert (TMLSID0: false = false); auto. apply TMLSID in TMLSID0; clear TMLSID.
+      assert (TMLB0: false = false); auto. apply TMLB in TMLB0; clear TMLB.
+      rewrite H0 in *. ss. des. clear TMLSID1. split; auto.
+      unfold Genv.perm_globvar in TMPERM. des_ifs. split.
+      2:{ unfold NW. lia. }
+      split; eauto. ss. apply Z.divide_0_r. }
+    { ss. }
+    { ss.
+      match goal with
+      | [ |- match_code _ _ _ ?i0 ?s0 ] =>
+        replace i0 with ((fun '(p, (le, _)) => itree_of_imp_ret sge le ms mn (p)) : (_ * (lenv * val)) -> _);
+          replace s0 with [exit_stmt]; eauto
+      end.
+      { econs 1. }
+      extensionality x. unfold itree_of_imp_ret, itree_of_imp_cont. grind. destruct p0. rewrite interp_imp_expr_Var. grind. }
+    { ss.
+      match goal with
+      | [ |- match_stack _ _ _ _ ?i0 ?s0 ] =>
+        replace i0 with ((itree_of_imp_pop_bottom ms mn) : (_ * (lenv * val)) -> _);
+          replace s0 with (Some ret_call_main); eauto
+      end.
+      { econs 1. }
+      extensionality x. unfold itree_of_imp_pop_bottom. grind. sim_red. Red.prw ltac:(_red_gen) 1 0. ss.
+    }
+  Qed.
+
+  Theorem single_compile_program_improves
+          (src: Imp.programL) (tgt: Csharpminor.program)
+          (WFPROG: incl (name1 src.(defsL)) ((name1 src.(prog_varsL)) ++ (name2 src.(prog_funsL))))
+          (WFPROG3: forall blk name,
+              let modl := ModL.add (Mod.lift (Mem (fun _ => false))) (ImpMod.get_modL src) in
+              let ge := (Sk.load_skenv (Sk.sort modl.(ModL.sk))) in
+              (ge.(SkEnv.blk2id) blk = Some name) -> call_ban name = false)
+          (WFPROG2 : forall gn gv, In (gn, Sk.Gvar gv) (Sk.sort (defsL src)) -> In (gn, gv) (prog_varsL src))
+          (COMP: Imp2Csharpminor.compile src = OK tgt)
+    :
+      <<IMPROVES: improves2_program (imp_sem src) (Csharpminor.semantics tgt)>>.
+  Proof.
+    red. unfold improves2_program. i. inv BEH.
+    { eapply single_compile_behavior_improves; eauto. }
+    (* initiall wrong case, for us only when main is not found *)
+    exists (Tr.ub). split; red; eauto.
+    2:{ pfold. econs 4; eauto.
+        - ss.
+        - unfold behavior_prefix. exists (Goes_wrong E0). ss.
+    }
+    rename H into NOINIT.
+    unfold imp_sem in *. ss. unfold ModSemL.initial_itr.
+    pfold. econs 6; ss; eauto.
+    unfold Beh.inter. ss. unfold assume. grind.
+    apply ModSemL.step_trigger_take_iff in STEP. des. clarify. split; eauto.
+    red. unfold ITree.map; ss.
+    unfold unwrapU. des_ifs.
+    (* main do not exists, ub *)
+    2:{ sim_red. unfold triggerUB. grind. econs 6; ss. grind. ss. apply ModSemL.step_trigger_take_iff in STEP. des. clarify. }
+
+    (* found main, contradiction *)
+    exfalso.
+    rename Heq into FSEM.
+    grind. rewrite alist_find_find_some in FSEM. rewrite find_map in FSEM.
+    match goal with
+    | [ FSEM: o_map (?a) _ = _ |- _ ] => destruct a eqn:FOUND; ss; clarify
+    end.
+    destruct p as [mn [fn ff]]; ss; clarify.
+    rewrite Sk.add_unit_l in FOUND.
+    eapply found_imp_function in FOUND. des; clarify.
+    hexploit in_tgt_prog_defs_ifuns; eauto. i.
+    des. rename H into COMPF. clear FOUND.
+    assert (COMPF2: In (compile_iFun (mn, ("main", ff))) (prog_defs tgt)); auto.
+    eapply Globalenvs.Genv.find_symbol_exists in COMPF.
+    destruct COMPF as [b TGTFG].
+    assert (TGTGFIND: Globalenvs.Genv.find_def (Globalenvs.Genv.globalenv tgt) b = Some (snd (compile_iFun (mn, ("main", ff))))).
+    { hexploit tgt_genv_find_def_by_blk; eauto. }
+
+    unfold compile in COMP. des_ifs.
+    match goal with [ H: Genv.find_symbol (Genv.globalenv ?_tgt) _ = _ |- _ ] => set (tgt:=_tgt) in * end.
+    hexploit (Genv.init_mem_exists tgt); eauto.
+    { i. subst tgt; ss. hexploit perm_elements_PTree_norepeat_in_in; eauto.
+      i. apply H0 in H. clear H0. apply decomp_gdefs in H. des; ss; clarify; eauto.
+      { unfold bts in BTS1. apply Coqlib.list_in_map_inv in BTS1. des. destruct fd; ss; clarify. destruct x0; ss; clarify. }
+      { destruct fd. unfold compile_eFun in SYS; ss; clarify. }
+      { destruct fd. unfold compile_eFun in EFS; ss; clarify. }
+      { depgen EVS. clear. i. unfold compile_eVar in EVS. ss; clarify. }
+      { depgen IFS. clear. i. destruct fd as [mn [fn ff]]. unfold compile_iFun in IFS; ss; clarify. }
+      { depgen IVS. clear. i. unfold compile_iVar in IVS. destruct vd; ss; clarify. split; ss; eauto.
+        - split; eauto. apply Z.divide_0_r.
+        - i. des; eauto; clarify. }
+    }
+    i. des. unfold compile_iFun in *; ss; clarify.
+    match goal with
+    | [ H: Genv.find_def _ _ = Some (Gfun ?_fdef) |- _ ] => set (fdef:=_fdef) in * end.
+    specialize NOINIT with (Callstate fdef [] Kstop m).
+    apply NOINIT.
+    econs; ss; eauto.
+    unfold Genv.find_funct_ptr. rewrite TGTGFIND. ss.
+  Qed.
+
+End PROOFSINGLE.
+
+
+
