clightlight/Clightlight2ClightSim.v
@@ -1,0 +1,84 @@
+From compcert Require Import Globalenvs Smallstep AST Integers Events Behaviors Errors Memory.
+Require Import Coqlib.
+Require Import ITreelib.
+Require Import Skeleton.
+Require Import PCM.
+Require Import STS Behavior.
+Require Import Any.
+Require Import ModSem.
+Require Import ConvC2ITree.
+Require Import SimSTS3.
+Require Import Clight_Mem0.
+Require Import IRed.
+From Ordinal Require Import Ordinal Arithmetic.
+
+(* Require Import Clightlight2ClightMatch.
+Require Import Clightlight2ClightArith. *)
+Require Import Clightlight2ClightGenv.
+(* Require Import Clightlight2ClightLenv.
+Require Import Clightlight2ClightMem. *)
+
+From compcert Require Import Clight Clightdefs.
+
+Lemma unbind_trigger E:
+  forall [X0 X1 A : Type] (ktr0 : X0 -> itree E A) (ktr1 : X1 -> itree E A) e0 e1,
+    (x <- trigger e0;; ktr0 x = x <- trigger e1;; ktr1 x) -> (X0 = X1 /\ e0 ~= e1 /\ ktr0 ~= ktr1).
+Proof.
+  i. eapply f_equal with (f:=_observe) in H. cbn in H.
+  inv H. split; auto.
+  dependent destruction H3. dependent destruction H2.
+  cbv in x. subst. split; auto.
+  assert (ktr0 = ktr1); clarify.
+  extensionality x. eapply equal_f in x0.
+  rewrite ! subst_bind in *.
+  irw in x0. eauto.
+Qed.
+
+Lemma angelic_step :
+  forall (X : Prop) (ktr next : itree eventE Any.t),
+    ModSemL.step (trigger (Take X);;; ktr) None next -> (next = ktr /\ X).
+Proof.
+  i. dependent destruction H; try (irw in x; clarify; fail).
+  rewrite <- bind_trigger in x. apply unbind_trigger in x.
+  des. clarify.
+Qed.
+
+(* Lemma eval_exprlist_length :
+  forall a b c d l1 l2
+    (EE: eval_exprlist a b c d l1 l2),
+    <<EELEN: List.length l1 = List.length l2>>.
+Proof.
+  i. induction EE; ss; clarify; eauto.
+Qed. *)
+
+  Ltac rewriter :=
+    try match goal with
+        | H: _ = _ |- _ => rewrite H in *; clarify
+        end.
+
+  Lemma Clight_wf_semantics types defs WF_TYPES
+    :
+      wf_semantics (semantics2 (mkprogram types defs (List.map (fun '(gn, _) => gn) defs) (ident_of_string "main") WF_TYPES)).
+  Proof.
+    econs.
+    { i. inv STEP0; inv STEP1; ss; rewriter.
+      { hexploit (@Csharpminor_eval_expr_determ a v v0); et. i. rewriter. }
+      { hexploit (@Csharpminor_eval_expr_determ addr vaddr vaddr0); et. i. rewriter.
+        hexploit (@Csharpminor_eval_expr_determ a v v0); et. i. rewriter. }
+      { hexploit (@Csharpminor_eval_expr_determ a vf vf0); et. i. rewriter.
+        hexploit (@Csharpminor_eval_exprlist_determ bl vargs vargs0); et. i. rewriter. }
+      { hexploit (@Csharpminor_eval_exprlist_determ bl vargs vargs0); et. i. rewriter.
+        hexploit external_call_determ; [eapply H0|eapply H12|..]. i. des.
+        inv H1. hexploit H2; et. i. des. clarify. }
+      { hexploit (@Csharpminor_eval_expr_determ a v v0); et. i. rewriter.
+        inv H0; inv H12; auto. }
+      { hexploit (@Csharpminor_eval_expr_determ a v v0); et. i. rewriter.
+        inv H0; inv H12; et. }
+      { hexploit (@Csharpminor_eval_expr_determ a v v0); et. i. rewriter. }
+      { hexploit (@alloc_variables_determ (fn_vars f) e e0); et. i. des; clarify. }
+      { hexploit external_call_determ; [eapply H|eapply H6|..]. i. des.
+        inv H0. hexploit H1; et. i. des. clarify. }
+    }
+    { i. inv FINAL. inv STEP. }
+    { i. inv FINAL0. inv FINAL1. ss. }
+  Qed.
