clightlight/ConvC2ITree.v
@@ -1,0 +1,1499 @@
+(* Require Import ZArith String List Lia. *)
+
+Require Import Coqlib.
+Require Import ITreelib.
+Require Import Skeleton.
+Require Import PCM.
+Require Import STS Behavior.
+Require Import Any.
+Require Import ModSem.
+Require Import AList.
+
+From compcert Require Import
+     AST Maps Globalenvs Memory Values Linking Integers.
+From compcert Require Import
+     Ctypes Clight Clightdefs.
+
+
+Global Program Instance EMSConfigC: EMSConfig := {|
+  finalize := fun rv =>
+                match rv↓ with
+                | Some (rv) =>
+                  match rv with
+                  | Vint z => Some z↑
+                  | _ => None
+                  end
+                | _ => None
+                end;
+  initial_arg := ([]: list val)↑;
+|}
+.
+Definition admit (excuse: String.string) {T: Type} : T.  Admitted.
+Tactic Notation "admit" constr(excuse) := idtac excuse; exact (admit excuse).
+
+Section GType.
+  
+  Inductive C_SkelEntry:=
+  | Cgfun (function_type: type)
+  | Cgvar (gv: globvar type)
+  .
+
+End GType.
+
+Section Clight.
+Context {eff : Type -> Type}.
+Context {HasCall : callE -< eff}.
+Context {HasEvent : eventE -< eff}.
+Variable sk: Sk.t.
+Let skenv: SkEnv.t := Sk.load_skenv sk.
+Variable ce: composite_env.
+  
+Section EVAL_EXPR_COMP.
+
+  Local Open Scope Z.
+  
+  Definition divide_c (n m: Z): bool :=
+    let x := m / n in
+    (x * n =? m).
+
+  Definition assign_loc_c (ce: composite_env)
+           (ty: type) (b: block) (ofs: ptrofs)
+           (v: val): itree eff unit :=
+  match access_mode ty with
+  | By_value chunk =>
+    ccallU "store" (chunk, Vptr b ofs, v)
+  | By_copy =>
+    match v with
+    | Vptr b' ofs' =>
+      let chk1 :=
+          if (0 <? sizeof ce ty) then
+            andb (divide_c
+                    (alignof_blockcopy ce ty)
+                    (Ptrofs.unsigned ofs'))
+                 (divide_c
+                    (alignof_blockcopy ce ty)
+                    (Ptrofs.unsigned ofs))
+          else true in
+      if negb chk1 then Ret tt else
+        let chk2 :=
+            (orb (negb (b' =? b))%positive
+                 (orb (Ptrofs.unsigned ofs' =? Ptrofs.unsigned ofs)
+                      (orb (Ptrofs.unsigned ofs' + sizeof ce ty <=? Ptrofs.unsigned ofs)
+                           (Ptrofs.unsigned ofs + sizeof ce ty <=? Ptrofs.unsigned ofs'))))%Z
+        in
+        if negb chk2 then Ret tt else
+          bytes <- @ccallU _ _ _ _ (option (list memval))
+                           "loadbytes" (Vptr b' ofs', sizeof ce ty);;
+          ccallU "storebytes" (Vptr b ofs, bytes)
+    | _ => Ret tt
+    end
+  | By_reference => Ret tt
+  | By_nothing => Ret tt
+  end.
+
+  Definition deref_loc_c (ty: type)
+             (b:block) (ofs: ptrofs): itree eff (option val) :=
+    match access_mode ty with
+    | By_value chunk => (v <- ccallU "load" (chunk, Vptr b ofs);; Ret(Some v) )
+    | By_reference => Ret (Some (Vptr b ofs))
+    | By_copy => Ret (Some (Vptr b ofs))
+    | By_nothing => Ret None
+    end.
+
+  Variable e: Clight.env.
+  Variable le: Clight.temp_env.
+
+  Section EVAL_LVALUE.
+    Variable _eval_expr_c: expr -> itree eff (option val).
+
+    Definition _eval_lvalue_c (a: expr)
+      : itree eff (option (block * (ptrofs * bitfield))) :=
+      match a with
+      | Evar id ty =>
+        match e ! id with
+        | Some (l, ty') =>
+          if type_eq ty ty' then Ret (Some (l, (Ptrofs.zero, Full)))
+          else Ret None
+        | None =>
+          match SkEnv.id2blk skenv (string_of_ident id) with
+          | Some i => Ret (Some (Pos.of_nat (S i), (Ptrofs.zero, Full)))
+          | None => Ret None
+          end
+        end
+      | Ederef a ty =>
+        v <- _eval_expr_c a;;
+        match v with
+        | Some (Vptr l ofs) => Ret (Some (l, (ofs, Full)))
+        | _ => Ret None
+        end
+      | Efield a i ty =>
+        v <- _eval_expr_c a;;
+        match v with
+        | Some (Vptr l ofs) =>
+          match Clight.typeof a with
+          | Tstruct id att =>
+            match ce ! id with
+            | Some co =>
+              match field_offset ce i (co_members co) with
+              | Errors.OK (delta, bf) =>
+                Ret (Some (l, (Ptrofs.add ofs (Ptrofs.repr delta), bf)))
+              | _ => Ret None
+              end
+            | _ => Ret None
+            end
+          | Tunion id att =>
+            match ce ! id with
+            | Some co =>
+                match union_field_offset ce i (co_members co) with
+                | Errors.OK (delta, bf) =>
+                    Ret (Some (l, ((Ptrofs.add ofs (Ptrofs.repr delta)), bf)))
+                | _ => Ret None
+                end
+            | None => Ret None
+            end
+          | _ => Ret None
+          end
+        | _ => Ret None
+        end
+      | _ => Ret None
+      end.
+
+  End EVAL_LVALUE.
+
+  Definition weak_valid_pointer_c (b: block) (ofs: Z): itree eff bool:=
+    b1 <- ccallU "valid_pointer" (b, ofs);;
+    b2 <- ccallU "valid_pointer" (b, (ofs - 1)%Z);;
+    Ret (b1 || b2).
+  
+  Definition bool_val_c v ty: itree eff (option bool) :=
+    match Cop.classify_bool ty with
+    | Cop.bool_case_i =>
+      match v with
+      | Vint n => Ret (Some (negb (Int.eq n Int.zero)))
+      | Vptr b ofs =>
+        if Archi.ptr64
+        then Ret None
+        else
+          ret <- weak_valid_pointer_c b (Ptrofs.unsigned ofs);;
+          if (ret: bool)
+          then Ret (Some true)
+          else Ret None
+      | _ => Ret None
+      end
+    | Cop.bool_case_l =>
+      match v with
+      | Vlong n => Ret (Some (negb (Int64.eq n Int64.zero)))
+      | Vptr b ofs =>
+        if negb Archi.ptr64
+        then Ret None
+        else
+          ret <- weak_valid_pointer_c b (Ptrofs.unsigned ofs);;
+          if (ret: bool)
+          then Ret (Some true)
+          else Ret None
+      | _ => Ret None
+      end
+    | Cop.bool_case_f =>
+      match v with
+      | Vfloat f => Ret (Some (negb (Floats.Float.cmp Ceq f Floats.Float.zero)))
+      | _ => Ret None
+      end
+    | Cop.bool_case_s =>
+      match v with
+      | Vsingle f => Ret (Some (negb (Floats.Float32.cmp Ceq f Floats.Float32.zero)))
+      | _ => Ret None
+      end
+    | Cop.bool_default => Ret None
+    end
+  .
+
+  Definition unary_op_c op v ty: itree eff (option val) :=
+    match op with
+    | Cop.Onotbool =>
+      v <- bool_val_c v ty;; Ret (Coqlib.option_map (Val.of_bool ∘ negb) v)
+    | Cop.Onotint => Ret (Cop.sem_notint v ty)
+    | Cop.Oneg => Ret (Cop.sem_neg v ty)
+    | Cop.Oabsfloat => Ret (Cop.sem_absfloat v ty)
+    end
+  .
+
+  Definition sem_cast_c v t1 t2: itree eff (option val) :=
+    match Cop.classify_cast t1 t2 with
+    | Cop.cast_case_pointer =>
+      match v with
+      | Vint _ => if Archi.ptr64 then Ret None else Ret (Some v)
+      | Vlong _ => if Archi.ptr64 then Ret (Some v) else Ret None
+      | Vptr _ _ => Ret (Some v)
+      | _ => Ret None
+      end
+    | Cop.cast_case_i2i sz2 si2 =>
+      match v with
+      | Vint i => Ret (Some (Vint (Cop.cast_int_int sz2 si2 i)))
+      | _ => Ret None
+      end
+    | Cop.cast_case_f2f =>
+      match v with
+      | Vfloat f => Ret (Some (Vfloat f))
+      | _ => Ret None
+      end
+    | Cop.cast_case_s2s =>
+      match v with
+      | Vsingle f => Ret (Some (Vsingle f))
+      | _ => Ret None
+      end
+    | Cop.cast_case_f2s =>
+      match v with
+      | Vfloat f => Ret (Some (Vsingle (Floats.Float.to_single f)))
+      | _ => Ret None
+      end
+    | Cop.cast_case_s2f =>
+      match v with
+      | Vsingle f => Ret (Some (Vfloat (Floats.Float.of_single f)))
+      | _ => Ret None
+      end
+    | Cop.cast_case_i2f si1 =>
+      match v with
+      | Vint i => Ret (Some (Vfloat (Cop.cast_int_float si1 i)))
+      | _ => Ret None
+      end
+    | Cop.cast_case_i2s si1 =>
+      match v with
+      | Vint i => Ret (Some (Vsingle (Cop.cast_int_single si1 i)))
+      | _ => Ret None
+      end
+    | Cop.cast_case_f2i sz2 si2 =>
+      match v with
+      | Vfloat f =>
+        match Cop.cast_float_int si2 f with
+        | Some i => Ret (Some (Vint (Cop.cast_int_int sz2 si2 i)))
+        | None => Ret None
+        end
+      | _ => Ret None
+      end
+    | Cop.cast_case_s2i sz2 si2 =>
+      match v with
+      | Vsingle f =>
+        match Cop.cast_single_int si2 f with
+        | Some i => Ret (Some (Vint (Cop.cast_int_int sz2 si2 i)))
+        | None => Ret None
+        end
+      | _ => Ret None
+      end
+    | Cop.cast_case_l2l =>
+      match v with
+      | Vlong n => Ret (Some (Vlong n))
+      | _ => Ret None
+      end
+    | Cop.cast_case_i2l si =>
+      match v with
+      | Vint n => Ret (Some (Vlong (Cop.cast_int_long si n)))
+      | _ => Ret None
+      end
+    | Cop.cast_case_l2i sz si =>
+      match v with
+      | Vlong n =>
+        Ret (Some (Vint (Cop.cast_int_int sz si (Int.repr (Int64.unsigned n)))))
+      | _ => Ret None
+      end
+    | Cop.cast_case_l2f si1 =>
+      match v with
+      | Vlong i => Ret (Some (Vfloat (Cop.cast_long_float si1 i)))
+      | _ => Ret None
+      end
+    | Cop.cast_case_l2s si1 =>
+      match v with
+      | Vlong i => Ret (Some (Vsingle (Cop.cast_long_single si1 i)))
+      | _ => Ret None
+      end
+    | Cop.cast_case_f2l si2 =>
+      match v with
+      | Vfloat f =>
+        match Cop.cast_float_long si2 f with
+        | Some i => Ret (Some (Vlong i))
+        | None => Ret None
+        end
+      | _ => Ret None
+      end
+    | Cop.cast_case_s2l si2 =>
+      match v with
+      | Vsingle f =>
+        match Cop.cast_single_long si2 f with
+        | Some i => Ret (Some (Vlong i))
+        | None => Ret None
+        end
+      | _ => Ret None
+      end
+    | Cop.cast_case_i2bool =>
+      match v with
+      | Vint n => Ret (Some (Vint (if Int.eq n Int.zero then Int.zero else Int.one)))
+      | Vptr b ofs =>
+        if Archi.ptr64
+        then Ret None
+        else
+          ret <- weak_valid_pointer_c b (Ptrofs.unsigned ofs);;
+          if (ret: bool)
+          then Ret (Some Vone)
+          else Ret None
+      | _ => Ret None
+      end
+    | Cop.cast_case_l2bool =>
+      match v with
+      | Vlong n =>
+        Ret (Some (Vint (if Int64.eq n Int64.zero then Int.zero else Int.one)))
+      | Vptr b ofs =>
+        if negb Archi.ptr64
+        then Ret None
+        else
+          ret <- weak_valid_pointer_c b (Ptrofs.unsigned ofs);;
+          if (ret: bool)
+          then Ret (Some Vone)
+          else Ret None
+      | _ => Ret None
+      end
+    | Cop.cast_case_f2bool =>
+      match v with
+      | Vfloat f =>
+        Ret (Some
+               (Vint
+                  (if Floats.Float.cmp Ceq f Floats.Float.zero
+                   then Int.zero
+                   else Int.one)))
+      | _ => Ret None
+      end
+    | Cop.cast_case_s2bool =>
+      match v with
+      | Vsingle f =>
+        Ret (Some
+               (Vint
+                  (if Floats.Float32.cmp Ceq f Floats.Float32.zero
+                   then Int.zero
+                   else Int.one)))
+      | _ => Ret None
+      end
+    | Cop.cast_case_struct id1 id2 | Cop.cast_case_union id1 id2 =>
+                                     match v with
+                                     | Vptr _ _ => if ident_eq id1 id2
+                                                   then Ret (Some v) else Ret None
+                                     | _ => Ret None
+                                     end
+    | Cop.cast_case_void => Ret (Some v)
+    | Cop.cast_case_default => Ret None
+    end.
+
+  Definition sem_binarith_c sem_int sem_long sem_float sem_single
+             v1 t1 v2 t2: itree eff (option val) :=
+    let c := Cop.classify_binarith t1 t2 in
+    let t := Cop.binarith_type c in
+    v1' <- sem_cast_c v1 t1 t;;
+    match v1' with
+    | Some v1' =>
+      v2' <- sem_cast_c v2 t2 t;;
+      match v2' with
+      | Some v2' =>
+        match c with
+        | Cop.bin_case_i sg =>
+          match v1' with
+          | Vint n1 =>
+            match v2' with
+            | Vint n2 => Ret (sem_int sg n1 n2)
+            | _ => Ret None
+            end
+          | _ => Ret None
+          end
+        | Cop.bin_case_l sg =>
+          match v1' with
+          | Vlong n1 =>
+            match v2' with
+            | Vlong n2 => Ret (sem_long sg n1 n2)
+            | _ => Ret None
+            end
+          | _ => Ret None
+          end
+        | Cop.bin_case_f =>
+          match v1' with
+          | Vfloat n1 =>
+            match v2' with
+            | Vfloat n2 => Ret (sem_float n1 n2)
+            | _ => Ret None
+            end
+          | _ => Ret None
+          end
+        | Cop.bin_case_s =>
+          match v1' with
+          | Vsingle n1 =>
+            match v2' with
+            | Vsingle n2 => Ret (sem_single n1 n2)
+            | _ => Ret None
+            end
+          | _ => Ret None
+          end
+        | Cop.bin_default => Ret None
+        end
+      | None => Ret None
+      end
+    | None => Ret None
+    end.
+
+  Definition sem_add_c cenv v1 t1 v2 t2: itree eff (option val) :=
+    match Cop.classify_add t1 t2 with
+    | Cop.add_case_pi ty si => Ret (Cop.sem_add_ptr_int cenv ty si v1 v2)
+    | Cop.add_case_pl ty => Ret (Cop.sem_add_ptr_long cenv ty v1 v2)
+    | Cop.add_case_ip si ty => Ret (Cop.sem_add_ptr_int cenv ty si v2 v1)
+    | Cop.add_case_lp ty => Ret (Cop.sem_add_ptr_long cenv ty v2 v1)
+    | Cop.add_default =>
+      sem_binarith_c
+        (fun (_ : signedness) (n1 n2 : int) => Some (Vint (Int.add n1 n2)))
+        (fun (_ : signedness) (n1 n2 : int64) => Some (Vlong (Int64.add n1 n2)))
+        (fun n1 n2 : Floats.float => Some (Vfloat (Floats.Float.add n1 n2)))
+        (fun n1 n2 : Floats.float32 =>
+           Some (Vsingle (Floats.Float32.add n1 n2))) v1 t1 v2 t2
+    end.
+
+  Definition sem_sub_c cenv v1 t1 v2 t2: itree eff (option val) :=
+    match Cop.classify_sub t1 t2 with
+    | Cop.sub_case_pi ty si =>
+      match v1 with
+      | Vint n1 =>
+        match v2 with
+        | Vint n2 =>
+          if Archi.ptr64
+          then Ret None
+          else
+            Ret (Some
+                   (Vint (Int.sub n1 (Int.mul (Int.repr (sizeof cenv ty)) n2))))
+        | _ => Ret None
+        end
+      | Vlong n1 =>
+        match v2 with
+        | Vint n2 =>
+          let n3 := Cop.cast_int_long si n2 in
+          if Archi.ptr64
+          then
+            Ret (Some
+                   (Vlong
+                      (Int64.sub n1 (Int64.mul (Int64.repr (sizeof cenv ty)) n3))))
+          else Ret None
+        | _ => Ret None
+        end
+      | Vptr b1 ofs1 =>
+        match v2 with
+        | Vint n2 =>
+          let n3 := Cop.ptrofs_of_int si n2 in
+          Ret (Some
+                 (Vptr b1
+                       (Ptrofs.sub ofs1
+                                   (Ptrofs.mul (Ptrofs.repr (sizeof cenv ty)) n3))))
+        | _ => Ret None
+        end
+      | _ => Ret None
+      end
+    | Cop.sub_case_pp ty =>
+      match v1 with
+      | Vptr b1 ofs1 =>
+        match v2 with
+        | Vptr b2 ofs2 =>
+          if eq_block b1 b2
+          then
+            let sz := sizeof cenv ty in
+            if
+              Coqlib.proj_sumbool (Coqlib.zlt 0 sz) &&
+              Coqlib.proj_sumbool (Coqlib.zle sz Ptrofs.max_signed)
+            then
+              Ret (Some
+                     (Vptrofs
+                        (Ptrofs.divs (Ptrofs.sub ofs1 ofs2) (Ptrofs.repr sz))))
+            else Ret None
+          else Ret None
+        | _ => Ret None
+        end
+      | _ => Ret None
+      end
+    | Cop.sub_case_pl ty =>
+      match v1 with
+      | Vint n1 =>
+        match v2 with
+        | Vlong n2 =>
+          let n3 := Int.repr (Int64.unsigned n2) in
+          if Archi.ptr64
+          then Ret None
+          else
+            Ret (Some
+                   (Vint (Int.sub n1 (Int.mul (Int.repr (sizeof cenv ty)) n3))))
+        | _ => Ret None
+        end
+      | Vlong n1 =>
+        match v2 with
+        | Vlong n2 =>
+          if Archi.ptr64
+          then
+            Ret (Some
+                   (Vlong
+                      (Int64.sub n1 (Int64.mul (Int64.repr (sizeof cenv ty)) n2))))
+          else Ret None
+        | _ => Ret None
+        end
+      | Vptr b1 ofs1 =>
+        match v2 with
+        | Vlong n2 =>
+          let n3 := Ptrofs.of_int64 n2 in
+          Ret (Some
+                 (Vptr b1
+                       (Ptrofs.sub ofs1
+                                   (Ptrofs.mul (Ptrofs.repr (sizeof cenv ty)) n3))))
+        | _ => Ret None
+        end
+      | _ => Ret None
+      end
+    | Cop.sub_default =>
+      sem_binarith_c
+        (fun (_ : signedness) (n1 n2 : int) => Some (Vint (Int.sub n1 n2)))
+        (fun (_ : signedness) (n1 n2 : int64) => Some (Vlong (Int64.sub n1 n2)))
+        (fun n1 n2 : Floats.float => Some (Vfloat (Floats.Float.sub n1 n2)))
+        (fun n1 n2 : Floats.float32 =>
+           Some (Vsingle (Floats.Float32.sub n1 n2))) v1 t1 v2 t2
+    end.
+
+  Definition sem_mul_c v1 t1 v2 t2: itree eff (option val) :=
+    sem_binarith_c
+      (fun (_ : signedness) (n1 n2 : int) => Some (Vint (Int.mul n1 n2)))
+      (fun (_ : signedness) (n1 n2 : int64) => Some (Vlong (Int64.mul n1 n2)))
+      (fun n1 n2 : Floats.float => Some (Vfloat (Floats.Float.mul n1 n2)))
+      (fun n1 n2 : Floats.float32 => Some (Vsingle (Floats.Float32.mul n1 n2)))
+      v1 t1 v2 t2.
+
+  Definition sem_div_c v1 t1 v2 t2: itree eff (option val) :=
+    sem_binarith_c
+      (fun (sg : signedness) (n1 n2 : int) =>
+         match sg with
+         | Signed =>
+           if
+             Int.eq n2 Int.zero
+             || Int.eq n1 (Int.repr Int.min_signed) && Int.eq n2 Int.mone
+           then None
+           else Some (Vint (Int.divs n1 n2))
+         | Unsigned =>
+           if Int.eq n2 Int.zero then None else Some (Vint (Int.divu n1 n2))
+         end)
+      (fun (sg : signedness) (n1 n2 : int64) =>
+         match sg with
+         | Signed =>
+           if
+             Int64.eq n2 Int64.zero
+             || Int64.eq n1 (Int64.repr Int64.min_signed) &&
+               Int64.eq n2 Int64.mone
+           then None
+           else Some (Vlong (Int64.divs n1 n2))
+         | Unsigned =>
+           if Int64.eq n2 Int64.zero
+           then None
+           else Some (Vlong (Int64.divu n1 n2))
+         end) (fun n1 n2 : Floats.float => Some (Vfloat (Floats.Float.div n1 n2)))
+      (fun n1 n2 : Floats.float32 => Some (Vsingle (Floats.Float32.div n1 n2)))
+      v1 t1 v2 t2.
+
+  Definition sem_mod_c v1 t1 v2 t2: itree eff (option val) :=
+    sem_binarith_c
+      (fun (sg : signedness) (n1 n2 : int) =>
+         match sg with
+         | Signed =>
+           if
+             Int.eq n2 Int.zero
+             || Int.eq n1 (Int.repr Int.min_signed) && Int.eq n2 Int.mone
+           then None
+           else Some (Vint (Int.mods n1 n2))
+         | Unsigned =>
+           if Int.eq n2 Int.zero then None else Some (Vint (Int.modu n1 n2))
+         end)
+      (fun (sg : signedness) (n1 n2 : int64) =>
+         match sg with
+         | Signed =>
+           if
+             Int64.eq n2 Int64.zero
+             || Int64.eq n1 (Int64.repr Int64.min_signed) &&
+               Int64.eq n2 Int64.mone
+           then None
+           else Some (Vlong (Int64.mods n1 n2))
+         | Unsigned =>
+           if Int64.eq n2 Int64.zero
+           then None
+           else Some (Vlong (Int64.modu n1 n2))
+         end) (fun _ _ : Floats.float => None) (fun _ _ : Floats.float32 => None)
+      v1 t1 v2 t2.
+  
+  Definition sem_and_c v1 t1 v2 t2: itree eff (option val) :=
+    sem_binarith_c
+      (fun (_ : signedness) (n1 n2 : int) => Some (Vint (Int.and n1 n2)))
+      (fun (_ : signedness) (n1 n2 : int64) => Some (Vlong (Int64.and n1 n2)))
+      (fun _ _ : Floats.float => None) (fun _ _ : Floats.float32 => None)
+      v1 t1 v2 t2.
+
+  Definition sem_or_c v1 t1 v2 t2: itree eff (option val) :=
+    sem_binarith_c
+      (fun (_ : signedness) (n1 n2 : int) => Some (Vint (Int.or n1 n2)))
+      (fun (_ : signedness) (n1 n2 : int64) => Some (Vlong (Int64.or n1 n2)))
+      (fun _ _ : Floats.float => None) (fun _ _ : Floats.float32 => None)
+      v1 t1 v2 t2.
+
+  Definition sem_xor_c v1 t1 v2 t2: itree eff (option val) :=
+    sem_binarith_c
+      (fun (_ : signedness) (n1 n2 : int) => Some (Vint (Int.xor n1 n2)))
+      (fun (_ : signedness) (n1 n2 : int64) => Some (Vlong (Int64.xor n1 n2)))
+      (fun _ _ : Floats.float => None) (fun _ _ : Floats.float32 => None)
+      v1 t1 v2 t2.
+
+  Definition cmplu_bool_c c v1 v2 : itree eff (option bool) :=
+    match v1 with
+    | Vlong n1 =>
+      match v2 with
+      | Vlong n2 => Ret (Some (Int64.cmpu c n1 n2))
+      | Vptr b2 ofs2 =>
+        if negb Archi.ptr64
+        then Ret None
+        else
+          ret <- weak_valid_pointer_c b2 (Ptrofs.unsigned ofs2);;
+          if
+            Int64.eq n1 Int64.zero && ret
+          then Ret (Val.cmp_different_blocks c)
+          else Ret None
+      | _ => Ret None
+      end
+    | Vptr b1 ofs1 =>
+      match v2 with
+      | Vlong n2 =>
+        if negb Archi.ptr64
+        then Ret None
+        else
+          ret <- weak_valid_pointer_c b1 (Ptrofs.unsigned ofs1);;
+          if
+            Int64.eq n2 Int64.zero && ret
+          then Ret (Val.cmp_different_blocks c)
+          else Ret None
+      | Vptr b2 ofs2 =>
+        if negb Archi.ptr64
+        then Ret None
+        else
+          if eq_block b1 b2
+          then
+            ret1 <- weak_valid_pointer_c b1 (Ptrofs.unsigned ofs1);;
+            ret2 <- weak_valid_pointer_c b2 (Ptrofs.unsigned ofs2);;
+            if
+              ret1 && ret2
+            then Ret (Some (Ptrofs.cmpu c ofs1 ofs2))
+            else Ret None
+          else
+            ret1 <- ccallU "valid_pointer" (b1, ofs1);;
+            ret2 <- ccallU "valid_pointer" (b2, ofs2);;
+            if
+              ret1 && ret2
+            then Ret (Val.cmp_different_blocks c)
+            else Ret None
+      | _ => Ret None
+      end
+    | _ => Ret None
+    end.
+
+  Definition cmpu_bool_c c v1 v2 : itree eff (option bool) :=
+    match v1 with
+    | Vint n1 =>
+      match v2 with
+      | Vint n2 => Ret (Some (Int.cmpu c n1 n2))
+      | Vptr b2 ofs2 =>
+        if negb Archi.ptr64
+        then Ret None
+        else
+          ret <- weak_valid_pointer_c b2 (Ptrofs.unsigned ofs2);;
+          if
+            Int.eq n1 Int.zero && ret
+          then Ret (Val.cmp_different_blocks c)
+          else Ret None
+      | _ => Ret None
+      end
+    | Vptr b1 ofs1 =>
+      match v2 with
+      | Vint n2 =>
+        if negb Archi.ptr64
+        then Ret None
+        else
+          ret <- weak_valid_pointer_c b1 (Ptrofs.unsigned ofs1);;
+          if
+            Int.eq n2 Int.zero && ret
+          then Ret (Val.cmp_different_blocks c)
+          else Ret None
+      | Vptr b2 ofs2 =>
+        if Archi.ptr64
+        then Ret None
+        else
+          if eq_block b1 b2
+          then
+            ret1 <- weak_valid_pointer_c b1 (Ptrofs.unsigned ofs1);;
+            ret2 <- weak_valid_pointer_c b2 (Ptrofs.unsigned ofs2);;
+            if
+              ret1 && ret2
+            then Ret (Some (Ptrofs.cmpu c ofs1 ofs2))
+            else Ret None
+          else
+            ret1 <- ccallU "valid_pointer" (b1, ofs1);;
+            ret2 <- ccallU "valid_pointer" (b2, ofs2);;
+            if
+              ret1 && ret2
+            then Ret (Val.cmp_different_blocks c)
+            else Ret None
+      | _ => Ret None
+      end
+    | _ => Ret None
+    end.
+
+  Definition cmp_ptr_c c v1 v2: itree eff (option val) :=
+    ret <- (if Archi.ptr64
+            then cmplu_bool_c c v1 v2
+            else cmpu_bool_c c v1 v2);;
+    Ret (Coqlib.option_map Val.of_bool ret).
+  
+  Definition sem_cmp_c c v1 t1 v2 t2: itree eff (option val) :=
+    match Cop.classify_cmp t1 t2 with
+    | Cop.cmp_case_pp => cmp_ptr_c c v1 v2
+    | Cop.cmp_case_pi si =>
+      match v2 with
+      | Vint n2 =>
+        let v2' := Vptrofs (Cop.ptrofs_of_int si n2) in
+        cmp_ptr_c c v1 v2'
+      | Vptr _ _ => if Archi.ptr64 then Ret None else cmp_ptr_c  c v1 v2
+      | _ => Ret None
+      end
+    | Cop.cmp_case_ip si =>
+      match v1 with
+      | Vint n1 =>
+        let v1' := Vptrofs (Cop.ptrofs_of_int si n1) in
+        cmp_ptr_c c v1' v2
+      | Vptr _ _ => if Archi.ptr64 then Ret None else cmp_ptr_c c v1 v2
+      | _ => Ret None
+      end
+    | Cop.cmp_case_pl =>
+      match v2 with
+      | Vlong n2 =>
+        let v2' := Vptrofs (Ptrofs.of_int64 n2) in cmp_ptr_c c v1 v2'
+      | Vptr _ _ => if Archi.ptr64 then cmp_ptr_c c v1 v2 else Ret None
+      | _ => Ret None
+      end
+    | Cop.cmp_case_lp =>
+      match v1 with
+      | Vlong n1 =>
+        let v1' := Vptrofs (Ptrofs.of_int64 n1) in cmp_ptr_c c v1' v2
+      | Vptr _ _ => if Archi.ptr64 then cmp_ptr_c c v1 v2 else Ret None
+      | _ => Ret None
+      end
+    | Cop.cmp_default =>
+      sem_binarith_c
+        (fun (sg : signedness) (n1 n2 : int) =>
+           Some
+             (Val.of_bool
+                match sg with
+                | Signed => Int.cmp c n1 n2
+                | Unsigned => Int.cmpu c n1 n2
+                end))
+        (fun (sg : signedness) (n1 n2 : int64) =>
+           Some
+             (Val.of_bool
+                match sg with
+                | Signed => Int64.cmp c n1 n2
+                | Unsigned => Int64.cmpu c n1 n2
+                end))
+        (fun n1 n2 : Floats.float =>
+           Some (Val.of_bool (Floats.Float.cmp c n1 n2)))
+        (fun n1 n2 : Floats.float32 =>
+           Some (Val.of_bool (Floats.Float32.cmp c n1 n2))) v1 t1 v2 t2
+    end.
+
+  Definition binary_op_c cenv op v1 t1 v2 t2: itree eff (option val) :=
+    match op with
+    | Cop.Oadd => sem_add_c cenv v1 t1 v2 t2
+    | Cop.Osub => sem_sub_c cenv v1 t1 v2 t2
+    | Cop.Omul => sem_mul_c v1 t1 v2 t2
+    | Cop.Odiv => sem_div_c v1 t1 v2 t2
+    | Cop.Omod => sem_mod_c v1 t1 v2 t2
+    | Cop.Oand => sem_and_c v1 t1 v2 t2
+    | Cop.Oor => sem_or_c v1 t1 v2 t2
+    | Cop.Oxor => sem_xor_c v1 t1 v2 t2
+    | Cop.Oshl => Ret (Cop.sem_shl v1 t1 v2 t2)
+    | Cop.Oshr => Ret (Cop.sem_shr v1 t1 v2 t2)
+    | Cop.Oeq => sem_cmp_c Ceq v1 t1 v2 t2
+    | Cop.One => sem_cmp_c Cne v1 t1 v2 t2
+    | Cop.Olt => sem_cmp_c Clt v1 t1 v2 t2
+    | Cop.Ogt => sem_cmp_c Cgt v1 t1 v2 t2
+    | Cop.Ole => sem_cmp_c Cle v1 t1 v2 t2
+    | Cop.Oge => sem_cmp_c Cge v1 t1 v2 t2
+    end.
+  
+  Fixpoint eval_expr_c (expr: Clight.expr): itree eff (option val) :=
+    match expr with
+    | Econst_int i ty => Ret (Some (Vint i))
+    | Econst_float f ty => Ret (Some (Vfloat f))
+    | Econst_single f ty => Ret (Some (Vsingle f))
+    | Econst_long i ty => Ret (Some (Vlong i))
+    | Etempvar id ty => Ret ((le ! id))
+    | Eaddrof a ty =>
+      v <- _eval_lvalue_c eval_expr_c a;;
+      match v with
+      | None => Ret None (*??*)
+      | Some (loc, (ofs, bf)) => Ret (Some (Vptr loc ofs))
+      end
+    | Eunop op a ty =>
+      v <- eval_expr_c a;;
+      match v with
+      | None => Ret None
+      | Some v1 =>
+        unary_op_c op v1 (Clight.typeof a)
+      end
+    | Ebinop op a1 a2 ty =>
+      v1 <- eval_expr_c a1;;
+      v2 <- eval_expr_c a2;;
+      match v1, v2 with
+      | Some v1, Some v2 =>
+        binary_op_c ce op
+                    v1 (Clight.typeof a1)
+                    v2 (Clight.typeof a2)
+      | _, _ => Ret None
+      end
+    | Ecast a ty =>
+      v <- eval_expr_c a;;
+      match v with
+      | None => Ret None
+      | Some v1 =>
+        sem_cast_c v1 (Clight.typeof a) ty
+      end
+    | Esizeof ty1 ty =>
+      Ret (Some (Vptrofs (Ptrofs.repr (sizeof ce ty1))))
+    | Ealignof ty1 ty =>
+      Ret (Some (Vptrofs (Ptrofs.repr (alignof ce ty1))))
+    | a =>
+      v <- _eval_lvalue_c eval_expr_c a;;
+      match v with
+      | None => Ret None
+      | Some (loc, (ofs, bf)) =>
+        v <- deref_loc_c (Clight.typeof a) loc ofs;; Ret v
+      end
+    end.
+
+
+  Definition eval_lvalue_c
+    : expr -> itree eff (option (block * (ptrofs * bitfield))) :=
+    _eval_lvalue_c eval_expr_c.
+
+  Fixpoint eval_exprlist_c
+           (es: list expr) (ts: typelist)
+    : itree eff (option (list val)) :=
+    match es, ts with
+    | [], Ctypes.Tnil =>
+        Ret (Some [])
+    | e::es', Ctypes.Tcons ty ts' =>
+      v1 <- eval_expr_c e;;
+      vs <- eval_exprlist_c es' ts';; 
+      match v1, vs with
+      | Some v1, Some vs =>
+        v2 <- sem_cast_c v1 (typeof e) ty;;
+        match v2 with
+        | Some v2 => Ret (Some (v2::vs))
+        | None => Ret None
+        end
+      | _, _ =>
+          Ret None
+      end
+    | _, _ => Ret None
+    end.
+
+End EVAL_EXPR_COMP.
+
+Definition id_list_norepet_c: list ident -> bool :=
+  fun ids => if Coqlib.list_norepet_dec (ident_eq) ids then true else false.
+
+Definition id_list_disjoint_c: list ident -> list ident -> bool :=
+  fun ids1 ids2 =>
+    if (Coqlib.list_disjoint_dec ident_eq ids1 ids2)
+    then true else false.
+
+Fixpoint alloc_variables_c (ce: composite_env) (e: env)
+         (vars: list (ident * type))
+  : itree eff env := 
+  match vars with
+  | [] => Ret e
+  | (id, ty) :: vars' =>
+    v <- ccallU "salloc" (0%Z, sizeof ce ty);;
+    match v with
+    | Vptr b ofs => alloc_variables_c ce (PTree.set id (b, ty) e) vars'
+    | _ => triggerUB
+    end
+  end.
+
+Definition function_entry_c
+           (ce: composite_env) (f: function) (vargs: list val)
+  : itree eff (option (env * temp_env)) :=
+  if (id_list_norepet_c (var_names (fn_vars f)) &&
+      id_list_norepet_c (var_names (fn_params f)) &&
+      id_list_disjoint_c (var_names (fn_params f))
+                         (var_names (fn_temps f)))%bool
+  then
+    e <- alloc_variables_c ce empty_env (fn_vars f);;
+    match
+      bind_parameter_temps (fn_params f) vargs
+                            (create_undef_temps
+                               (fn_temps f))
+    with
+    | None => Ret None
+    | Some le => Ret
+
+ (Some (e, le))
+    end
+  else Ret None.
+
+Section DECOMP.
+
+  Notation itr_t :=
+    (itree eff (env * temp_env *
+                option bool (*break/continue*) * option val)).
+
+  Definition _sassign_c e le a1 a2 :=
+    v <- eval_lvalue_c e le a1;;
+    match v with
+    | Some (loc, (ofs, bf)) =>
+      v2 <- eval_expr_c e le a2;; 
+      match v2 with
+      | Some v2 =>
+        v <- sem_cast_c v2 (typeof a2) (typeof a1);;
+        match v with
+        | Some v =>
+          assign_loc_c ce (typeof a1) loc ofs v
+        | None => Ret tt
+        end
+      | None => Ret tt
+      end
+    | None => Ret tt
+    end.
+
+  Definition _scall_c e le a al
+    : itree eff val :=
+    match Cop.classify_fun (typeof a) with
+    | Cop.fun_case_f tyargs tyres cconv =>
+      vf <- (eval_expr_c e le a);;
+      vf <- vf?;;
+      vargs <- eval_exprlist_c e le al tyargs;;
+      vargs <- vargs?;;
+      match vf with
+      | Vptr b ofs =>
+          '(gsym, skentry) <- (nth_error sk (pred (Pos.to_nat b)))?;;
+          gd <- (skentry↓)?;;
+          fd <- (match gd with Cgfun fd => Some fd | _ => None end)?;;
+          if type_eq fd
+               (Tfunction tyargs tyres cconv)
+          then ccallU gsym vargs
+          else triggerUB
+      | _ => triggerUB (* unreachable b*)
+      end
+    | _ => triggerUB
+    end.
+
+  Definition _site_c
+             (e: env) (le: temp_env) (a: expr)
+    : itree eff (option bool) :=
+    v1 <- eval_expr_c e le a;;
+    match v1 with
+    | Some v1 =>
+      bool_val_c v1 (typeof a)
+    | None => Ret None
+    end.
+
+  Definition sloop_iter_body_one
+             (itr: itr_t)
+    : itree eff (env * temp_env * (option (option val))) :=
+    '(e', le', obc, v) <- itr;;
+    match v with
+    | Some retv =>
+      (* return *)
+      Ret (e', le', Some (Some retv))
+    | None =>
+      if (* is_break *)
+        match obc with
+        | None => false
+        | Some bc => bc
+        end
+      then
+        (* break, not return *)
+        Ret (e', le', Some None)
+      else
+        (* continue *)
+        Ret (e', le', None)
+    end.
+
+  Definition sloop_iter_body_two
+             (itr: itr_t)
+    : itree eff (env * temp_env * (option (option val))) :=
+    '(e', le', obc, v) <- itr;;
+    match v with
+    | Some retv =>
+      (* return *)
+      Ret (e', le', Some (Some retv))
+    | None =>
+      if (* is_break *)
+        match obc with
+        | None => false
+        | Some bc => bc
+        end
+      then
+        (* break, not return *)
+        Ret (e', le', Some None)
+      else
+        (* continue *)
+        Ret (e', le', None)
+    end.
+
+  Definition sloop_iter_body
+             (itr1 itr2: env -> temp_env -> itr_t)
+             (i: env * temp_env)
+    : itree eff
+            (env * temp_env +
+             env * temp_env * option val) :=
+    let '(e, le) := i in
+    (* '(e1, le1, m1, obc1, v1) <- itr1 e le m ;; *)
+    '(e1, le1, ov1) <- sloop_iter_body_one (itr1 e le) ;;
+    match ov1 with
+    | Some v1 =>
+      (* break or return *)
+      Ret (inr (e1, le1, v1))
+    | None =>
+      (* run loop2 *)
+      '(e2, le2, ov2) <- sloop_iter_body_two (itr2 e1 le1);;
+      match ov2 with
+      | Some v2 =>
+        Ret (inr (e2, le2, v2))
+      | None =>
+        Ret (inl (e2, le2))
+      end
+    end.
+
+  Definition _sloop_itree
+             (e: env) (le: temp_env)
+             (itr1 itr2: env -> temp_env -> itr_t)
+    : itr_t :=
+    '(e', le', v) <-
+    ITree.iter (sloop_iter_body itr1 itr2) (e, le) ;;
+    Ret (e', le', None, v).
+
+  Fixpoint free_list_aux (l: list (block * Z * Z)): itree eff unit :=
+    match l with
+    | nil => Ret tt
+    | (b, lo, hi):: l' =>
+      @ccallU _ _ _ _ unit "sfree" (b, lo, hi);;;
+      free_list_aux l'
+    end.
+
+  Definition block_of_binding (ce: composite_env) (id_b_ty: ident * (block * type)) :=
+    let (_, p) := id_b_ty in let (b, ty) := p in (b, 0%Z, sizeof ce ty).
+
+  Definition blocks_of_env (ce: composite_env) :=
+    List.map (block_of_binding ce) ∘ PTree.elements.
+  
+  Definition _sreturn_c
+             (retty: type)
+             (e: env) (le: temp_env)
+             (oa: option expr)
+    : itree eff (option val) :=
+    free_list_aux (blocks_of_env ce e);;;
+    match oa with
+    | None => Ret (Some Vundef)
+    | Some a =>
+      v <- eval_expr_c e le a;;
+      match v with
+      | None => Ret None
+      | Some v =>
+        sem_cast_c v (typeof a) retty
+      end
+    end.
+
+  Fixpoint decomp_stmt
+           (retty: type)
+           (stmt: statement) (* (k: cont) *)
+           (e: env) (le: temp_env)
+    : itr_t :=
+    match stmt with
+    | Sskip =>
+      Ret ((* k, *) e, le, None, None)
+    | Sassign a1 a2 =>
+      _sassign_c e le a1 a2;;;
+      Ret (e, le, None, None)
+    | Sset id a =>
+      v <- eval_expr_c e le a ;;
+      match v with
+      | Some v =>
+        let le' := PTree.set id v le in
+        Ret (e, le', None, None)
+      | None =>
+        triggerUB
+      end
+    | Scall optid a al =>
+        v <- _scall_c e le a al;;
+        Ret (e, (set_opttemp optid v le), None, None)
+    | Sbuiltin optid ef targs el => triggerUB
+    | Ssequence s1 s2 =>
+      '(e', le', bc, v) <- decomp_stmt retty s1 e le;;
+      match v with
+      | Some retval =>
+        Ret (e', le', None, v)
+      | None =>
+        match bc with
+        | None =>
+          decomp_stmt retty s2 e' le'
+        | Some _ =>
+          Ret (e', le', bc, None)
+        end
+      end
+    | Sifthenelse a s1 s2 =>
+      b <- _site_c e le a;;
+      match b with
+      | Some b =>
+        if (b: bool) then (decomp_stmt retty s1 e le)
+        else (decomp_stmt retty s2 e le)
+      | None =>
+        triggerUB
+      end
+    | Sloop s1 s2 =>
+      let itr1 := decomp_stmt retty s1 in
+      let itr2 := decomp_stmt retty s2 in
+      _sloop_itree e le itr1 itr2
+    (* '(e, le, m, bc, v) <- itr ;; *)
+
+    | Sbreak =>
+      Ret (e, le, Some true, None)
+    | Scontinue =>
+      Ret (e, le, Some false, None)
+    | Sreturn oa =>
+      v <- _sreturn_c retty e le oa;;
+      match v with
+      | Some v =>
+        Ret (e, le, None, Some v)
+      | None =>
+        triggerUB
+      end
+    | _ =>
+      (* not supported *)
+      triggerUB
+    end.
+
+  Definition decomp_func
+           (f: Clight.function)
+           (vargs: list val)
+    : itree eff val :=
+    t <- function_entry_c ce f vargs;;
+    match t with
+    | None => triggerUB
+    | Some (e, le) =>
+      '(_, _, c, ov) <- decomp_stmt (fn_return f) (fn_body f) e le;; c?;;;
+      let v := match ov with
+               | None => Vundef
+               | Some v => v
+               end
+      in
+      Ret v
+    end.
+
+End DECOMP.
+End Clight.
+(* Notation call_data := (block * (* fundef * *) list val * mem)%type. *)
+
+(* Section TRANS. *)
+
+(*   (* Variable cprog_app: Clight.program. *) *)
+(*   Variable global_definitions : list (ident * globdef fundef type). *)
+(*   Variable public_idents : list ident. *)
+(*   Let defined_names := List.map fst global_definitions. *)
+
+(*   Fixpoint filter_dec_not {A: Type} {P: A -> Prop} (f: forall x: A, {P x} + {~ P x}) (l: list A) : list A := *)
+(*     match l with *)
+(*     | nil => nil *)
+(*     | x :: l' => if f x then filter_dec_not f l' else x :: (filter_dec_not f l') *)
+(*     end. *)
+  
+(*   Definition in_public x := in_dec Pos.eq_dec x public_idents. *)
+  
+(*   Definition rest_names := filter_dec_not in_public defined_names. *)
+
+(*   Definition in_rest x := in_dec Pos.eq_dec x rest_names. *)
+
+(*   Variable src_name : string.   (* source code file name *) *)
+
+(*   Definition prefix_pos pos := ident_of_string (src_name ++ "." ++ (string_of_ident pos))%string. *)
+
+(*   Definition rpl_pos pos := if in_rest pos then prefix_pos pos else pos. *)
+
+(*   Definition rpl_glob := List.map (fun x => (rpl_pos (fst x), snd x)) global_definitions. *)
+  
+(*   Fixpoint rpl_expr (e: expr) := *)
+(*     match e with *)
+(*     | Econst_int _ _ | Econst_float _ _ | Econst_single _ _ *)
+(*     | Econst_long _ _ | Etempvar _ _ | Esizeof _ _ | Ealignof _ _ => e *)
+(*     | Evar id ty => Evar (rpl_pos id) ty *)
+(*     | Ederef e' ty => Ederef (rpl_expr e') ty *)
+(*     | Eaddrof e' ty => Eaddrof (rpl_expr e') ty *)
+(*     | Eunop uop e' ty => Eunop uop (rpl_expr e') ty *)
+(*     | Ebinop bop e1 e2 ty => Ebinop bop (rpl_expr e1) (rpl_expr e2) ty *)
+(*     | Ecast e' ty => Ecast (rpl_expr e') ty *)
+(*     | Efield e' id ty => Efield (rpl_expr e') id ty *)
+(*     end. *)
+  
+(*   Fixpoint rpl_body (s : statement) := *)
+(*     match s with *)
+(*     | Sskip | Sbreak | Scontinue | Sgoto _ => s *)
+(*     | Sassign a1 a2 => Sassign (rpl_expr a1) (rpl_expr a2) *)
+(*     | Sset id a => Sset (rpl_pos id) (rpl_expr a) *)
+(*     | Scall optid a al => *)
+(*         Scall *)
+(*           (option_rec (fun _ => _) (Some ∘ rpl_pos) None optid) *)
+(*           (rpl_expr a) (List.map rpl_expr al) *)
+(*     | Sbuiltin optid ef targs el => *)
+(*         Sbuiltin *)
+(*           (option_rec (fun _ => _) (Some ∘ rpl_pos) None optid) *)
+(*           ef targs (List.map rpl_expr el) *)
+(*     | Ssequence s1 s2 => Ssequence (rpl_body s1) (rpl_body s2) *)
+(*     | Sifthenelse a s1 s2 => Sifthenelse (rpl_expr a) (rpl_body s1) (rpl_body s2) *)
+(*     | Sloop s1 s2 => Sloop (rpl_body s1) (rpl_body s2) *)
+(*     | Sreturn oa => Sreturn (option_rec (fun _ => _) (Some ∘ (rpl_expr)) None oa) *)
+(*     | Sswitch a ls => Sswitch (rpl_expr a) (rpl_labeled_stmt ls) *)
+(*     | Slabel l s => Slabel l (rpl_body s) *)
+(*     end *)
+      
+(*   with rpl_labeled_stmt (ls: labeled_statements) := *)
+(*          match ls with *)
+(*          | LSnil => LSnil *)
+(*          | LScons optz s ls' => LScons optz (rpl_body s) (rpl_labeled_stmt ls') *)
+(*          end. *)
+  
+(*   Definition trans_func (f: function) := *)
+(*     mkfunction f.(fn_return) f.(fn_callconv) f.(fn_params) f.(fn_vars) f.(fn_temps) (rpl_body f.(fn_body)). *)
+
+(*   Definition trans_initval (ii : init_data) := *)
+(*     match ii with *)
+(*     | Init_addrof id ofs => Init_addrof (rpl_pos id) ofs *)
+(*     | _ => ii *)
+(*     end. *)
+
+(*   Definition trans_var (gv: globvar type) := *)
+(*     {| *)
+(*       gvar_info := gv.(gvar_info); *)
+(*       gvar_init := List.map trans_initval gv.(gvar_init); *)
+(*       gvar_readonly := gv.(gvar_readonly); *)
+(*       gvar_volatile := gv.(gvar_volatile); *)
+(*     |} *)
+(*   . *)
+
+(*   Definition trans_global_def (g_def: globdef fundef type) := *)
+(*     match g_def with *)
+(*     | Gvar gv => Gvar (trans_var gv) *)
+(*     | Gfun (Internal f) => Gfun (Internal (trans_func f)) *)
+(*     | _ => g_def *)
+(*     end. *)
+
+
+(*   Definition trans_global_defs (g_defs: list (ident * globdef fundef type)) := *)
+(*     List.map (fun x => (rpl_pos (fst x), trans_global_def (snd x))) g_defs. *)
+
+(*   (* Program Definition append_srcname : Clight.program :=  *) *)
+(*   (*   {| *) *)
+(*   (*     prog_defs := trans_global_defs global_definitions; *) *)
+(*   (*     prog_public := public_idents; *) *)
+(*   (*     prog_main := cprog_app.(prog_main); *) *)
+(*   (*     prog_types := cprog_app.(prog_types); *) *)
+(*   (*     prog_comp_env := cprog_app.(prog_comp_env); *) *)
+(*   (*   |}. *) *)
+(*   (* Next Obligation. destruct cprog_app;auto. Qed. *) *)
+
+(* End TRANS. *)
+
+(* Section SITE_APP. *)
+(*   (* for site specific execution *) *)
+(*   (* not for proof *) *)
+(*   Import EventsL. *)
+
+(*   Definition sname := string. *)
+(*   Variable sn: sname. *)
+(*   Variable shared_fun_list: list gname. *)
+
+(*   Let is_shared_fun fn := in_dec string_dec fn shared_fun_list. *)
+
+(*   Definition site_append_morph_1 : Es ~> Es. (* for site specific module *) *)
+(*   Proof. *)
+(*     intros. destruct X. *)
+(*     { destruct c. destruct (is_shared_fun fn). *)
+(*       - exact (inl1 (Call mn fn args)). *)
+(*       - exact (inl1 (Call mn (sn ++ "." ++ fn) args)). } *)
+(*     destruct s. *)
+(*     { destruct s. *)
+(*       { destruct (is_shared_fun fn). *)
+(*         - exact (inr1 (inl1 (Spawn fn args))). *)
+(*         - exact (inr1 (inl1 (Spawn (sn ++ "." ++ fn) args))). } *)
+(*       exact (inr1 (inl1 Yield)). *)
+(*       exact (inr1 (inl1 Getpid)). *)
+(*       exact (inr1 (inl1 Getsn)). } *)
+(*     destruct s. *)
+(*     { destruct p. *)
+(*       - exact (inr1 (inr1 (inl1 (PPut (sn ++ "." ++ mn) p)))). *)
+(*       - exact (inr1 (inr1 (inl1 (PGet (sn ++ "." ++ mn))))). } *)
+(*     { destruct e. *)
+(*       exact (inr1 (inr1 (inr1 (Choose X)))). *)
+(*       exact (inr1 (inr1 (inr1 (Take X)))). *)
+(*       exact (inr1 (inr1 (inr1 (Syscall fn args rvs)))). } *)
+(*   Defined. *)
+  
+(*   Definition site_append_morph_2 (sn': sname) : Es ~> Es. (* for shared module *) *)
+(*   Proof. *)
+(*     intros. destruct X. *)
+(*     { destruct c. destruct (is_shared_fun fn). *)
+(*       - exact (inl1 (Call mn fn args)). *)
+(*       - exact (inl1 (Call mn (sn' ++ "." ++ fn) args)). } *)
+(*     destruct s. *)
+(*     { destruct s. *)
+(*       { destruct (is_shared_fun fn). *)
+(*         - exact (inr1 (inl1 (Spawn fn args))). *)
+(*         - exact (inr1 (inl1 (Spawn (sn' ++ "." ++ fn) args))). } *)
+(*       exact (inr1 (inl1 Yield)). *)
+(*       exact (inr1 (inl1 Getpid)). *)
+(*       exact (inr1 (inl1 Getsn)). *)
+(*     } *)
+(*     destruct s. *)
+(*     { destruct p. *)
+(*       - exact (inr1 (inr1 (inl1 (PPut mn p)))). *)
+(*       - exact (inr1 (inr1 (inl1 (PGet mn)))). } *)
+(*     { destruct e. *)
+(*       exact (inr1 (inr1 (inr1 (Choose X)))). *)
+(*       exact (inr1 (inr1 (inr1 (Take X)))). *)
+(*       exact (inr1 (inr1 (inr1 (Syscall fn args rvs)))). } *)
+(*   Defined. *)
+    
+
+(*   Definition site_appended_itree_1 : itree Es ~> itree Es := translate site_append_morph_1. *)
+(*   Definition site_appended_itree_2 (sn': sname) : itree Es ~> itree Es := translate (site_append_morph_2 sn'). *)
+
+(*   Definition append_site_1 (ms: ModSemL.t) : ModSemL.t := *)
+(*     {| *)
+(*       ModSemL.fnsems := List.map (fun '(gn, fnsem) => *)
+(*                        ((sn ++ "." ++ gn)%string, fun x => site_appended_itree_1 _ (fnsem x))) ms.(ModSemL.fnsems); *)
+(*       ModSemL.initial_mrs := List.map (map_fst (fun mn => (sn ++ "." ++ mn)%string)) ms.(ModSemL.initial_mrs); *)
+(*     |} *)
+(*   . *)
+
+(*   Definition append_caller_site {X Y: Type} (body: X -> itree Es Y) := *)
+(*     fun x => sn' <- trigger Getsn;; site_appended_itree_2 sn' _ (body x). *)
+
+(*   Definition append_site_2 (ms: ModSemL.t) : ModSemL.t := *)
+(*     {| *)
+(*       ModSemL.fnsems := List.map *)
+(*                           (fun '(gn, fnsem) => (gn, append_caller_site fnsem)) ms.(ModSemL.fnsems); *)
+(*       ModSemL.initial_mrs := ms.(ModSemL.initial_mrs); *)
+(*     |} *)
+(*   . *)
+
+(* End SITE_APP. *)
+
+
+Section DECOMP_PROG.
+
+  (* Context `{SystemEnv}. *)
+  Variable types: list composite_definition.
+  Variable defs: list (ident * globdef Clight.fundef type).
+  Variable public: list ident.
+  Variable wf: wf_composites types.
+  Let ce: composite_env := let (ce, _) := build_composite_env' types wf in ce.
+  
+  Variable mn: string.
+
+  (* Fixpoint get_source_name (filename : string) := *)
+  (*   String.substring 0 (String.length filename - 2) filename. *)
+
+  Fixpoint decomp_fundefs (sk: Sk.t)
+           (defs: list (ident * globdef Clight.fundef type))
+    : list (ident * (list val -> itree Es val)) :=
+    match defs with
+    | [] => []
+    | (id, gdef) :: defs' =>
+      match gdef with
+      | Gvar _ => decomp_fundefs sk defs'
+      | Gfun fd =>
+        match fd with
+        | Internal f => (id, decomp_func sk ce f) :: decomp_fundefs sk defs'
+        | _ => decomp_fundefs sk defs'
+        end
+      end
+    end.
+
+  Fixpoint get_sk (defs: list (ident * globdef Clight.fundef type)) :=
+    match defs with
+    | [] => []
+    | (id, gdef) :: defs' =>
+        match gdef with
+        | Gvar gv =>
+            match gv.(gvar_init) with
+            | [] => get_sk defs'
+            | _ => (string_of_ident id, (Cgvar gv)↑) :: get_sk defs'
+            end
+        | Gfun gf =>
+            match gf with
+            | Internal f => (string_of_ident id, (Cgfun (type_of_function f))↑) :: get_sk defs'
+            | _ => get_sk defs'
+            end
+        end
+    end
+  .
+
+  Definition modsem (sk: Sk.t) : ModSem.t := {|
+    ModSem.fnsems := List.map (fun '(fn, f) => (string_of_ident fn, cfunU f)) (decomp_fundefs sk defs);
+    ModSem.mn := mn;
+    ModSem.initial_st := tt↑;
+  |}.
+
+  Definition get_mod : Mod.t := {|
+    Mod.get_modsem := modsem;
+    Mod.sk := get_sk defs;
+  |}.
+
+End DECOMP_PROG.
+
+(* Section EXECUTION_STRUCTURE. *)
+(*   (*   execution modules consist of modules executes in sites independently  *) *)
+(*   (*   and modules accessable in every sites. *) *)
+(*   (* ------------------------------------------------------------------------ *) *)
+(*   (* example *) *)
+(*   (* site A : A1 A2 A3 *) *)
+(*   (* site B : B1 B2 B3 *) *)
+(*   (* shared : C1 C2 C3 *) *)
+(*   (* f: function append site name in local state and its own function *) *)
+(*   (* g: function append current site name in site specific function (so, its site name dynamically determined) *) *)
+(*   (* A's ModSemL: f (MemA + A1 + A2 + A3) <_ (enclose) skel of site A and shared *) *)
+(*   (* B's ModSemL: f (MemB + B1 + B2 + B3) <_ (enclose) skel of site B and shared *) *)
+(*   (* shared's ModSemL: g (C1 + C2 + C3) <_(enclose) skel of site A and site B and shared *) *)
+
+(*   Fixpoint remove_mult_name (l : Sk.t) : Sk.t := *)
+(*     match l with *)
+(*       | [] => [] *)
+(*       | (gn, gd)::xs => if in_dec string_dec gn (List.map fst xs) then remove_mult_name xs else (gn, gd)::(remove_mult_name xs) *)
+(*     end. *)
+
+(*   (* for skeleton padding *) *)
+(*   Definition sk_padmod (sk: Sk.t) := ModL.mk ModL.empty.(ModL.get_modsem) sk. *)
+
+(*   (* get one site's ModSemL *) *)
+(*   Definition proc_gen (shared_module: ModL.t) : sname * list Mod.t -> ModSemL.t := *)
+(*     fun '(sn, modlist) => *)
+(*       (append_site_1 sn (List.map fst shared_module.(ModL.enclose).(ModSemL.fnsems)) *)
+(*          (ModL.enclose (ModL.add (Mod.add_list modlist) (sk_padmod shared_module.(ModL.sk))))). *)
+  
+(*   (* turns exec_profile into one ModSemL *) *)
+(*   Definition sum_of_site_modules_view (exec_profile: list (sname * list Mod.t)) (shared_module: ModL.t) : ModSemL.t := *)
+(*     List.fold_left ModSemL.add (List.map (proc_gen shared_module) exec_profile) (ModSemL.mk [] []). *)
+
+(*   (* get all skeletons in sites and concat *) *)
+(*   Definition sum_of_site_skeletons (exec_profile: list (sname * list Mod.t)) : Sk.t := *)
+(*       remove_mult_name (List.concat (List.map (fun '(sn, modlist) => (Mod.add_list modlist).(ModL.sk)) exec_profile)). *)
+
+(*   (* turn shared modules into one ModSemL *) *)
+(*   Definition view_shared_module (exec_profile: list (sname * list Mod.t)) (shared_module: ModL.t) : ModSemL.t := *)
+(*     append_site_2 (List.map fst shared_module.(ModL.enclose).(ModSemL.fnsems)) *)
+(*       (ModL.enclose (ModL.add shared_module (sk_padmod (sum_of_site_skeletons exec_profile)))). *)
+  
+(* End EXECUTION_STRUCTURE. *)
